src/QueryStructure/Automation/AutoDB.v
@@ -49,11 +49,11 @@ Ltac lmap A f seq :=
       end
   in aux seq.
 
-  Require Import ADTNotation.BuildComputationalADT.
-  Require Import ADT.ComputationalADT.
+Require Import ADTNotation.BuildComputationalADT.
+Require Import ADT.ComputationalADT.
 
-  Ltac FullySharpenEachMethod delegateSigs delegateSpecs cRep' cAbsR' :=
-    match goal with
+Ltac FullySharpenEachMethod delegateSigs delegateSpecs cRep' cAbsR' :=
+  match goal with
       |- Sharpened (@BuildADT ?Rep ?consSigs ?methSigs ?consDefs ?methDefs) =>
       ilist_of_evar
         (ilist (fun nadt => ComputationalADT.cADT (namedADTSig nadt)) delegateSigs)
@@ -79,761 +79,761 @@ Ltac lmap A f seq :=
                                delegateSpecs
                                cAbsR')));
         unfold Dep_Type_BoundedIndex_app_comm_cons
-    end; simpl; repeat split.
+  end; simpl; repeat split.
 
-  Fixpoint Build_IndexedQueryStructure_Impl_Sigs
-    {indices : list NamedSchema}
-      (Index : ilist (fun ns : NamedSchema => SearchUpdateTerms (schemaHeading (relSchema ns))) indices)
-    : list NamedADTSig :=
-    match indices as indices return ilist _ indices -> list NamedADTSig with
-      | nil => fun _ => nil
-      | cons ns indices' =>
-        fun Index =>
-          {| ADTSigname := relName ns;
-             namedADTSig :=
-               BagSig (@Tuple (schemaHeading (relSchema ns))) (BagSearchTermType (ilist_hd Index)) (BagUpdateTermType (ilist_hd Index)) |}
-                       :: @Build_IndexedQueryStructure_Impl_Sigs indices' (ilist_tl Index)
-    end Index.
+Fixpoint Build_IndexedQueryStructure_Impl_Sigs
+         {indices : list NamedSchema}
+         (Index : ilist (fun ns : NamedSchema => SearchUpdateTerms (schemaHeading (relSchema ns))) indices)
+: list NamedADTSig :=
+  match indices as indices return ilist _ indices -> list NamedADTSig with
+    | nil => fun _ => nil
+    | cons ns indices' =>
+      fun Index =>
+        {| ADTSigname := relName ns;
+           namedADTSig :=
+             BagSig (@Tuple (schemaHeading (relSchema ns))) (BagSearchTermType (ilist_hd Index)) (BagUpdateTermType (ilist_hd Index)) |}
+          :: @Build_IndexedQueryStructure_Impl_Sigs indices' (ilist_tl Index)
+  end Index.
 
-  Fixpoint Build_IndexedQueryStructure_Impl_Specs
-           {indices : list NamedSchema}
-           (Index : ilist (fun ns : NamedSchema => SearchUpdateTerms (schemaHeading (relSchema ns))) indices)
-  : ilist (fun ns => ADT (namedADTSig ns)) (@Build_IndexedQueryStructure_Impl_Sigs indices Index) :=
-    match indices as indices return
-          forall (Index : ilist _ indices),
-            ilist (fun ns : NamedADTSig => ADT (namedADTSig ns))
-                  (@Build_IndexedQueryStructure_Impl_Sigs indices Index)
-    with
-      | nil => fun _ => inil _
-      | cons ns indices' =>
-        fun Index => icons {| ADTSigname := relName ns;
-                              namedADTSig := _ |}
-                           (@BagSpec (@Tuple (schemaHeading (relSchema ns)))
-                                     (BagSearchTermType (ilist_hd Index))
-                                     (BagUpdateTermType (ilist_hd Index))
-                                     (BagMatchSearchTerm (ilist_hd Index))
-                                     (BagApplyUpdateTerm (ilist_hd Index)))
-                           (@Build_IndexedQueryStructure_Impl_Specs indices' (ilist_tl Index))
-    end Index.
+Fixpoint Build_IndexedQueryStructure_Impl_Specs
+         {indices : list NamedSchema}
+         (Index : ilist (fun ns : NamedSchema => SearchUpdateTerms (schemaHeading (relSchema ns))) indices)
+: ilist (fun ns => ADT (namedADTSig ns)) (@Build_IndexedQueryStructure_Impl_Sigs indices Index) :=
+  match indices as indices return
+        forall (Index : ilist _ indices),
+          ilist (fun ns : NamedADTSig => ADT (namedADTSig ns))
+                (@Build_IndexedQueryStructure_Impl_Sigs indices Index)
+  with
+    | nil => fun _ => inil _
+    | cons ns indices' =>
+      fun Index => icons {| ADTSigname := relName ns;
+                            namedADTSig := _ |}
+                         (@BagSpec (@Tuple (schemaHeading (relSchema ns)))
+                                   (BagSearchTermType (ilist_hd Index))
+                                   (BagUpdateTermType (ilist_hd Index))
+                                   (BagMatchSearchTerm (ilist_hd Index))
+                                   (BagApplyUpdateTerm (ilist_hd Index)))
+                         (@Build_IndexedQueryStructure_Impl_Specs indices' (ilist_tl Index))
+  end Index.
 
- Fixpoint unroll_ilist {A} {B : A -> Type}
-           (As : list A)
-           (il : ilist B As)
-  : ilist B As :=
-    match As return ilist _ As -> ilist B As with
-      | nil => fun il => inil _
-      | a :: As' =>
-        fun il' => icons a (ilist_hd il') (unroll_ilist (ilist_tl il'))
-    end il.
+Fixpoint unroll_ilist {A} {B : A -> Type}
+         (As : list A)
+         (il : ilist B As)
+: ilist B As :=
+  match As return ilist _ As -> ilist B As with
+    | nil => fun il => inil _
+    | a :: As' =>
+      fun il' => icons a (ilist_hd il') (unroll_ilist (ilist_tl il'))
+  end il.
 
-  Definition Build_IndexedQueryStructure_Impl_cRep
+Definition Build_IndexedQueryStructure_Impl_cRep
            {indices : list NamedSchema}
            (Index : ilist (fun ns : NamedSchema => SearchUpdateTerms (schemaHeading (relSchema ns))) indices)
            (DelegateImpls : ilist (fun ns => cADT (namedADTSig ns)) (@Build_IndexedQueryStructure_Impl_Sigs indices Index))
-  : Type
-    :=
+: Type
+  :=
     i2list
       (fun (ns : NamedADTSig)
            (index : cADT (namedADTSig ns)) => cRep index) DelegateImpls.
 
-  Fixpoint map_IndexedQS_idx_boundi
-        {indices}
-  : forall
-      n
-      (Index : ilist
-                 (fun ns : NamedSchema =>
-                    SearchUpdateTerms (schemaHeading (relSchema ns)))
-                 indices)
-      idx,
-      nth_error
-        (map ADTSigname (Build_IndexedQueryStructure_Impl_Sigs Index))
-        n = Some idx
-      ->  nth_error (map relName indices) n = Some idx.
-  Proof.
-    refine (match indices with
-              | nil => _
-              | ns :: indices' =>
-                fun n =>
-                  match n return
-                        forall
-                          (Index : ilist
-                                     (fun ns : NamedSchema =>
-                                        SearchUpdateTerms (schemaHeading (relSchema ns)))
-                                     (ns :: indices'))
-                          idx,
-                          nth_error (map ADTSigname (Build_IndexedQueryStructure_Impl_Sigs Index)) n =
-                          Some idx ->
-                          nth_error (map relName (ns :: indices')) n = Some idx
-                  with
-                    | 0 => fun Index idx nth_n => nth_n
-                    | S n' => fun Index => (map_IndexedQS_idx_boundi indices' n' (ilist_tl Index))
-                  end
-            end);
-    simpl; intros; try discriminate; eauto.
-  Defined.
+Fixpoint map_IndexedQS_idx_boundi
+         {indices}
+: forall
+    n
+    (Index : ilist
+               (fun ns : NamedSchema =>
+                  SearchUpdateTerms (schemaHeading (relSchema ns)))
+               indices)
+    idx,
+    nth_error
+      (map ADTSigname (Build_IndexedQueryStructure_Impl_Sigs Index))
+      n = Some idx
+    ->  nth_error (map relName indices) n = Some idx.
+Proof.
+  refine (match indices with
+            | nil => _
+            | ns :: indices' =>
+              fun n =>
+                match n return
+                      forall
+                        (Index : ilist
+                                   (fun ns : NamedSchema =>
+                                      SearchUpdateTerms (schemaHeading (relSchema ns)))
+                                   (ns :: indices'))
+                        idx,
+                        nth_error (map ADTSigname (Build_IndexedQueryStructure_Impl_Sigs Index)) n =
+                        Some idx ->
+                        nth_error (map relName (ns :: indices')) n = Some idx
+                with
+                  | 0 => fun Index idx nth_n => nth_n
+                  | S n' => fun Index => (map_IndexedQS_idx_boundi indices' n' (ilist_tl Index))
+                end
+          end);
+  simpl; intros; try discriminate; eauto.
+Defined.
 
-  Definition map_IndexedQS_idx
-             indices
-             (Index : ilist (fun ns : NamedSchema => SearchUpdateTerms (schemaHeading (relSchema ns))) indices )
-             (idx : BoundedIndex
-                      (map ADTSigname
-                           (Build_IndexedQueryStructure_Impl_Sigs Index)))
-  : BoundedIndex (map relName indices) :=
-    {| bindex := bindex idx;
-       indexb := {| ibound := ibound (indexb idx);
-                    boundi := map_IndexedQS_idx_boundi _ Index (boundi (indexb idx))|} |}.
+Definition map_IndexedQS_idx
+           indices
+           (Index : ilist (fun ns : NamedSchema => SearchUpdateTerms (schemaHeading (relSchema ns))) indices )
+           (idx : BoundedIndex
+                    (map ADTSigname
+                         (Build_IndexedQueryStructure_Impl_Sigs Index)))
+: BoundedIndex (map relName indices) :=
+  {| bindex := bindex idx;
+     indexb := {| ibound := ibound (indexb idx);
+                  boundi := map_IndexedQS_idx_boundi _ Index (boundi (indexb idx))|} |}.
 
-  Fixpoint map_IndexedQS_idx_boundi'
-        {indices}
-  : forall
-      n
-      (Index : ilist
-                 (fun ns : NamedSchema =>
-                    SearchUpdateTerms (schemaHeading (relSchema ns)))
-                 indices)
-      idx,
-      nth_error (map relName indices) n = Some idx
-      -> nth_error
-        (map ADTSigname (Build_IndexedQueryStructure_Impl_Sigs Index))
-        n = Some idx.
-  Proof.
-    refine (match indices with
-              | nil => _
-              | ns :: indices' =>
-                fun n =>
-                  match n return
-                        forall
-                          (Index : ilist
-                                     (fun ns : NamedSchema =>
-                                        SearchUpdateTerms (schemaHeading (relSchema ns)))
-                                     (ns :: indices'))
-                          idx,
-                          nth_error (map relName (ns :: indices')) n = Some idx
-                          -> nth_error (map ADTSigname (Build_IndexedQueryStructure_Impl_Sigs Index)) n = Some idx
-                  with
-                    | 0 => fun Index idx nth_n => nth_n
-                    | S n' => fun Index => (map_IndexedQS_idx_boundi' indices' n' (ilist_tl Index))
-                  end
-            end);
-    simpl; intros; try discriminate; eauto.
-  Defined.
+Fixpoint map_IndexedQS_idx_boundi'
+         {indices}
+: forall
+    n
+    (Index : ilist
+               (fun ns : NamedSchema =>
+                  SearchUpdateTerms (schemaHeading (relSchema ns)))
+               indices)
+    idx,
+    nth_error (map relName indices) n = Some idx
+    -> nth_error
+         (map ADTSigname (Build_IndexedQueryStructure_Impl_Sigs Index))
+         n = Some idx.
+Proof.
+  refine (match indices with
+            | nil => _
+            | ns :: indices' =>
+              fun n =>
+                match n return
+                      forall
+                        (Index : ilist
+                                   (fun ns : NamedSchema =>
+                                      SearchUpdateTerms (schemaHeading (relSchema ns)))
+                                   (ns :: indices'))
+                        idx,
+                        nth_error (map relName (ns :: indices')) n = Some idx
+                        -> nth_error (map ADTSigname (Build_IndexedQueryStructure_Impl_Sigs Index)) n = Some idx
+                with
+                  | 0 => fun Index idx nth_n => nth_n
+                  | S n' => fun Index => (map_IndexedQS_idx_boundi' indices' n' (ilist_tl Index))
+                end
+          end);
+  simpl; intros; try discriminate; eauto.
+Defined.
 
-  Definition map_IndexedQS_idx'
-             indices
-             (Index : ilist (fun ns : NamedSchema => SearchUpdateTerms (schemaHeading (relSchema ns))) indices )
-             (idx : BoundedIndex (map relName indices))
-  : BoundedIndex
-                      (map ADTSigname
-                           (Build_IndexedQueryStructure_Impl_Sigs Index)) :=
-    {| bindex := bindex idx;
-       indexb := {| ibound := ibound (indexb idx);
-                    boundi := map_IndexedQS_idx_boundi' _ Index (boundi (indexb idx))|} |}.
+Definition map_IndexedQS_idx'
+           indices
+           (Index : ilist (fun ns : NamedSchema => SearchUpdateTerms (schemaHeading (relSchema ns))) indices )
+           (idx : BoundedIndex (map relName indices))
+: BoundedIndex
+    (map ADTSigname
+         (Build_IndexedQueryStructure_Impl_Sigs Index)) :=
+  {| bindex := bindex idx;
+     indexb := {| ibound := ibound (indexb idx);
+                  boundi := map_IndexedQS_idx_boundi' _ Index (boundi (indexb idx))|} |}.
 
-  Lemma ith_Build_IndexedQueryStructure_Impl_Sigs_eq
-        {indices}
-  : forall
-      (Index : ilist (fun ns : NamedSchema => SearchUpdateTerms (schemaHeading (relSchema ns))) indices )
-      (idx : BoundedIndex
-               (map ADTSigname
-                    (Build_IndexedQueryStructure_Impl_Sigs Index))),
-      (BagSig (@Tuple (schemaHeading (relSchema ((nth_Bounded relName indices (map_IndexedQS_idx Index idx))))))
-              (BagSearchTermType
-                 (ith_Bounded relName Index (map_IndexedQS_idx Index idx)))
-              (BagUpdateTermType
-                 (ith_Bounded relName Index (map_IndexedQS_idx Index idx))))
-      = namedADTSig
-          (nth_Bounded ADTSigname (Build_IndexedQueryStructure_Impl_Sigs Index) idx).
-  Proof.
-    destruct idx as [idx [n nth_n]].
-    revert Index idx n nth_n.
-    induction indices; destruct n; simpl; intros; try discriminate; eauto.
-    eapply (IHindices (ilist_tl Index) idx n nth_n).
-  Defined.
+Lemma ith_Build_IndexedQueryStructure_Impl_Sigs_eq
+      {indices}
+: forall
+    (Index : ilist (fun ns : NamedSchema => SearchUpdateTerms (schemaHeading (relSchema ns))) indices )
+    (idx : BoundedIndex
+             (map ADTSigname
+                  (Build_IndexedQueryStructure_Impl_Sigs Index))),
+    (BagSig (@Tuple (schemaHeading (relSchema ((nth_Bounded relName indices (map_IndexedQS_idx Index idx))))))
+            (BagSearchTermType
+               (ith_Bounded relName Index (map_IndexedQS_idx Index idx)))
+            (BagUpdateTermType
+               (ith_Bounded relName Index (map_IndexedQS_idx Index idx))))
+    = namedADTSig
+        (nth_Bounded ADTSigname (Build_IndexedQueryStructure_Impl_Sigs Index) idx).
+Proof.
+  destruct idx as [idx [n nth_n]].
+  revert Index idx n nth_n.
+  induction indices; destruct n; simpl; intros; try discriminate; eauto.
+  eapply (IHindices (ilist_tl Index) idx n nth_n).
+Defined.
 
-  Lemma ith_Build_IndexedQueryStructure_Impl_Specs_eq
-        {indices}
-  : forall
-      (Index : ilist (fun ns : NamedSchema => SearchUpdateTerms (schemaHeading (relSchema ns))) indices )
-      (idx : BoundedIndex
-               (map ADTSigname
-                    (Build_IndexedQueryStructure_Impl_Sigs Index))),
-      ith_Bounded ADTSigname (Build_IndexedQueryStructure_Impl_Specs Index) idx =
-  eq_rect _ ADT
-          (@BagSpec (@Tuple (schemaHeading (relSchema (@nth_Bounded NamedSchema string relName
-                                                                    indices (map_IndexedQS_idx Index idx)))))
-                    (BagSearchTermType (ith_Bounded _ Index (map_IndexedQS_idx Index idx)))
-                    (BagUpdateTermType (ith_Bounded _ Index (map_IndexedQS_idx Index idx)))
-                    (BagMatchSearchTerm (ith_Bounded _ Index (map_IndexedQS_idx Index idx)))
-                    (BagApplyUpdateTerm (ith_Bounded _ Index (map_IndexedQS_idx Index idx))))
-                    _ (ith_Build_IndexedQueryStructure_Impl_Sigs_eq Index idx).
-  Proof.
-    destruct idx as [idx [n nth_n]].
-    revert Index idx n nth_n.
-    induction indices; destruct n; simpl; intros; try discriminate; eauto.
-    eapply (IHindices (ilist_tl Index) idx n nth_n).
-  Defined.
+Lemma ith_Build_IndexedQueryStructure_Impl_Specs_eq
+      {indices}
+: forall
+    (Index : ilist (fun ns : NamedSchema => SearchUpdateTerms (schemaHeading (relSchema ns))) indices )
+    (idx : BoundedIndex
+             (map ADTSigname
+                  (Build_IndexedQueryStructure_Impl_Sigs Index))),
+    ith_Bounded ADTSigname (Build_IndexedQueryStructure_Impl_Specs Index) idx =
+    eq_rect _ ADT
+            (@BagSpec (@Tuple (schemaHeading (relSchema (@nth_Bounded NamedSchema string relName
+                                                                      indices (map_IndexedQS_idx Index idx)))))
+                      (BagSearchTermType (ith_Bounded _ Index (map_IndexedQS_idx Index idx)))
+                      (BagUpdateTermType (ith_Bounded _ Index (map_IndexedQS_idx Index idx)))
+                      (BagMatchSearchTerm (ith_Bounded _ Index (map_IndexedQS_idx Index idx)))
+                      (BagApplyUpdateTerm (ith_Bounded _ Index (map_IndexedQS_idx Index idx))))
+            _ (ith_Build_IndexedQueryStructure_Impl_Sigs_eq Index idx).
+Proof.
+  destruct idx as [idx [n nth_n]].
+  revert Index idx n nth_n.
+  induction indices; destruct n; simpl; intros; try discriminate; eauto.
+  eapply (IHindices (ilist_tl Index) idx n nth_n).
+Defined.
 
-  Definition map_IndexedQS_Rep
-             {indices}
-             (Index : ilist (fun ns : NamedSchema => SearchUpdateTerms (schemaHeading (relSchema ns))) indices )
-             idx
-             (rep : @IndexedEnsemble
-                      (@Tuple
-                         (schemaHeading
-                            (relSchema
-                               (@nth_Bounded NamedSchema string relName
-                                             indices (map_IndexedQS_idx Index idx) )))))
-  : Rep
-      (ith_Bounded ADTSigname
-                   (Build_IndexedQueryStructure_Impl_Specs Index) idx).
-  Proof.
-    destruct idx as [idx [n nth_n]].
-    revert Index idx n nth_n rep.
-    induction indices; destruct n; simpl; intros; try discriminate; eauto.
-    eapply IHindices; eauto.
-  Defined.
-
-  Definition map_IndexedQS_Rep'
-             {indices}
-             (Index : ilist (fun ns : NamedSchema => SearchUpdateTerms (schemaHeading (relSchema ns))) indices )
-             idx
-             (rep : Rep
-                      (ith_Bounded ADTSigname
-                                   (Build_IndexedQueryStructure_Impl_Specs Index)
-                                   (map_IndexedQS_idx' Index idx)))
-  : @IndexedEnsemble
-      (@Tuple
-         (schemaHeading
-            (relSchema
-               (@nth_Bounded NamedSchema string relName
-                             indices idx )))).
-  Proof.
-    destruct idx as [idx [n nth_n]].
-    revert Index idx n nth_n rep.
-    induction indices; destruct n; simpl; intros; try discriminate; eauto.
-    eapply (IHindices (ilist_tl Index)); eauto.
-  Defined.
-
-  Definition Build_IndexedQueryStructure_Impl_AbsR
-             {qs_schema : QueryStructureSchema}
-             (Index : ilist (fun ns : NamedSchema => SearchUpdateTerms (schemaHeading (relSchema ns))) (qschemaSchemas qs_schema) )
-             (DelegateImpls : ilist (fun ns => cADT (namedADTSig ns))
-                                     (Build_IndexedQueryStructure_Impl_Sigs Index))
-             (ValidImpl :
-                forall idx,
-                  refineADT (ith_Bounded ADTSigname
-                                         (Build_IndexedQueryStructure_Impl_Specs Index) idx)
-                            (LiftcADT (ith_Bounded ADTSigname DelegateImpls idx)))
-             (r_o : IndexedQueryStructure qs_schema Index)
-             (r_n : Build_IndexedQueryStructure_Impl_cRep Index DelegateImpls)
-  : Prop :=
-    forall idx,
-      AbsR (ValidImpl idx)
-           (map_IndexedQS_Rep Index idx (GetIndexedRelation r_o (map_IndexedQS_idx Index idx)))
-           (i2th_Bounded ADTSigname r_n idx).
-
-  Definition map_IndexedQS_Rep''
-             {indices}
-             (Index : ilist (fun ns : NamedSchema => SearchUpdateTerms (schemaHeading (relSchema ns))) indices )
-             idx
-             (rep : @IndexedEnsemble
-                      (@Tuple
-                         (schemaHeading
-                            (relSchema
-                               (@nth_Bounded NamedSchema string relName
-                                             indices idx)))))
-  : Rep
-      (ith_Bounded ADTSigname
-                   (Build_IndexedQueryStructure_Impl_Specs Index) (map_IndexedQS_idx' Index idx)).
-  Proof.
-    destruct idx as [idx [n nth_n]].
-    revert Index idx n nth_n rep.
-    induction indices; destruct n; simpl; intros; try discriminate; eauto.
-    eapply IHindices; eauto.
-  Defined.
-
-  Definition Build_IndexedQueryStructure_Impl_AbsR''
-             {qs_schema : QueryStructureSchema}
-             (Index : ilist (fun ns : NamedSchema => SearchUpdateTerms (schemaHeading (relSchema ns))) (qschemaSchemas qs_schema) )
-             (DelegateImpls : ilist (fun ns => cADT (namedADTSig ns))
-                                     (Build_IndexedQueryStructure_Impl_Sigs Index))
-             (ValidImpl :
-                forall idx : BoundedIndex (map relName (qschemaSchemas qs_schema)),
-                  refineADT (ith_Bounded ADTSigname
-                                         (Build_IndexedQueryStructure_Impl_Specs Index) (map_IndexedQS_idx' Index idx))
-                            (LiftcADT (ith_Bounded ADTSigname _ (map_IndexedQS_idx' Index idx))))
-             (r_o : IndexedQueryStructure qs_schema Index)
-             (r_n : Build_IndexedQueryStructure_Impl_cRep Index DelegateImpls)
-  : Prop :=
-    forall idx,
-      AbsR (ValidImpl idx)
-           (map_IndexedQS_Rep'' Index idx (GetIndexedRelation r_o idx))
-           (i2th_Bounded ADTSigname r_n (map_IndexedQS_idx' Index idx)).
-
-  Definition CallBagImplMethod
-             {qs_schema : QueryStructureSchema}
-             (Index : ilist (fun ns : NamedSchema => SearchUpdateTerms (schemaHeading (relSchema ns))) (qschemaSchemas qs_schema) )
-             (DelegateImpls : ilist (fun ns => cADT (namedADTSig ns))
-                                    (Build_IndexedQueryStructure_Impl_Sigs Index))
-             idx midx
-             (r_n : Build_IndexedQueryStructure_Impl_cRep Index DelegateImpls) :=
-    cMethods (ith_Bounded ADTSigname _ idx) midx (i2th_Bounded _ r_n idx).
-
-  Definition CallBagImplConstructor
-             {qs_schema : QueryStructureSchema}
-             (Index : ilist (fun ns : NamedSchema => SearchUpdateTerms (schemaHeading (relSchema ns))) (qschemaSchemas qs_schema) )
-             (DelegateImpls : ilist (fun ns => cADT (namedADTSig ns))
-                                    (Build_IndexedQueryStructure_Impl_Sigs Index))
-             idx midx :=
-    cConstructors (ith_Bounded ADTSigname DelegateImpls idx) midx .
-
-  Fixpoint Build_IndexedQueryStructure_Impl_midx
+Definition map_IndexedQS_Rep
            {indices}
-           (P : ADTSig -> Type)
-  : forall (Index : ilist (fun ns : NamedSchema => SearchUpdateTerms (schemaHeading (relSchema ns))) indices)
-             ridx
-             (midx : P
-                       (BagSig (@Tuple (schemaHeading
-                            (relSchema
-                               (@nth_Bounded NamedSchema string relName
-                                             indices (map_IndexedQS_idx Index ridx ) ))))
-                               (BagSearchTermType
-                                  (ith_Bounded relName Index (map_IndexedQS_idx Index ridx)))
-                               (BagUpdateTermType
-                                  (ith_Bounded relName Index (map_IndexedQS_idx Index ridx))))),
-      P
-        (namedADTSig
-           (nth_Bounded ADTSigname (Build_IndexedQueryStructure_Impl_Sigs Index)
-                        ridx)) :=
-    match indices return
-          forall (Index : ilist
-                            (fun ns : NamedSchema =>
-                               SearchUpdateTerms (schemaHeading (relSchema ns)))
-                            indices)
-                 (ridx : BoundedIndex
-                           (map ADTSigname (Build_IndexedQueryStructure_Impl_Sigs Index)))
-                 (midx : P
-                       (BagSig (@Tuple (schemaHeading
-                            (relSchema
-                               (@nth_Bounded NamedSchema string relName
-                                             indices (map_IndexedQS_idx Index ridx ) ))))
-                               (BagSearchTermType
-                                  (ith_Bounded relName Index (map_IndexedQS_idx Index ridx)))
-                               (BagUpdateTermType
-                                  (ith_Bounded relName Index (map_IndexedQS_idx Index ridx))))),
-      P
-        (namedADTSig
-           (nth_Bounded ADTSigname (Build_IndexedQueryStructure_Impl_Sigs Index)
-                        ridx))
-    with
-      | nil => fun _ ridx => BoundedIndex_nil _ ridx
-      | ns :: indices' =>
-        fun Index ridx =>
-          match ridx with
-            | {| bindex := ridx;
-                 indexb := {|ibound := n;
-                             boundi := nth_n |}|} =>
-              match n return
-                    forall
-                      (Index' : ilist
-                                  (fun ns : NamedSchema =>
-                                     SearchUpdateTerms (schemaHeading (relSchema ns))) (ns :: indices'))
-                      ridx nth_n,
-                      let idx := {| bindex := ridx;
-                                    indexb := {|ibound := n;
-                                                boundi := nth_n |}|} in
-                      P
-                                (BagSig (@Tuple (schemaHeading
-                                                   (relSchema
-                                                      (@nth_Bounded NamedSchema string relName
-                                                                    (ns :: indices') (map_IndexedQS_idx Index' idx ) ))))
-                                        (BagSearchTermType
-                                           (ith_Bounded relName Index' (map_IndexedQS_idx Index' idx)))
-                                        (BagUpdateTermType
-                                           (ith_Bounded relName Index' (map_IndexedQS_idx Index' idx)))) ->
-                      P
-                        (namedADTSig
-                           (nth_Bounded ADTSigname (Build_IndexedQueryStructure_Impl_Sigs Index')
-                                        {| bindex := ridx;
-                                           indexb := {|ibound := n;
-                                                       boundi := nth_n |}|}))
-              with
-                | 0 => fun Index idx nth_n midx => midx
-                | S n' => fun Index idx nth_n midx =>
-                            (@Build_IndexedQueryStructure_Impl_midx
-                               indices' P (ilist_tl Index)
-                               {| bindex := idx;
-                                  indexb := {|ibound := n';
-                                              boundi := nth_n |}|}
-                               midx)
-              end Index ridx nth_n
-                            end
-         end.
+           (Index : ilist (fun ns : NamedSchema => SearchUpdateTerms (schemaHeading (relSchema ns))) indices )
+           idx
+           (rep : @IndexedEnsemble
+                    (@Tuple
+                       (schemaHeading
+                          (relSchema
+                             (@nth_Bounded NamedSchema string relName
+                                           indices (map_IndexedQS_idx Index idx) )))))
+: Rep
+    (ith_Bounded ADTSigname
+                 (Build_IndexedQueryStructure_Impl_Specs Index) idx).
+Proof.
+  destruct idx as [idx [n nth_n]].
+  revert Index idx n nth_n rep.
+  induction indices; destruct n; simpl; intros; try discriminate; eauto.
+  eapply IHindices; eauto.
+Defined.
 
-  Definition Build_IndexedQueryStructure_Impl_MethodDom
+Definition map_IndexedQS_Rep'
            {indices}
-  : forall (Index : ilist (fun ns : NamedSchema => SearchUpdateTerms (schemaHeading (relSchema ns))) indices)
-           ridx
-           midx,
-      fst (MethodDomCod
-             (BagSig (@Tuple (schemaHeading (relSchema (nth_Bounded relName indices  ridx))))
-                     (BagSearchTermType
-                        (ith_Bounded relName Index ridx))
-                     (BagUpdateTermType
-                        (ith_Bounded relName Index ridx)))
-             midx)
+           (Index : ilist (fun ns : NamedSchema => SearchUpdateTerms (schemaHeading (relSchema ns))) indices )
+           idx
+           (rep : Rep
+                    (ith_Bounded ADTSigname
+                                 (Build_IndexedQueryStructure_Impl_Specs Index)
+                                 (map_IndexedQS_idx' Index idx)))
+: @IndexedEnsemble
+    (@Tuple
+       (schemaHeading
+          (relSchema
+             (@nth_Bounded NamedSchema string relName
+                           indices idx )))).
+Proof.
+  destruct idx as [idx [n nth_n]].
+  revert Index idx n nth_n rep.
+  induction indices; destruct n; simpl; intros; try discriminate; eauto.
+  eapply (IHindices (ilist_tl Index)); eauto.
+Defined.
+
+Definition Build_IndexedQueryStructure_Impl_AbsR
+           {qs_schema : QueryStructureSchema}
+           (Index : ilist (fun ns : NamedSchema => SearchUpdateTerms (schemaHeading (relSchema ns))) (qschemaSchemas qs_schema) )
+           (DelegateImpls : ilist (fun ns => cADT (namedADTSig ns))
+                                  (Build_IndexedQueryStructure_Impl_Sigs Index))
+           (ValidImpl :
+              forall idx,
+                refineADT (ith_Bounded ADTSigname
+                                       (Build_IndexedQueryStructure_Impl_Specs Index) idx)
+                          (LiftcADT (ith_Bounded ADTSigname DelegateImpls idx)))
+           (r_o : IndexedQueryStructure qs_schema Index)
+           (r_n : Build_IndexedQueryStructure_Impl_cRep Index DelegateImpls)
+: Prop :=
+  forall idx,
+    AbsR (ValidImpl idx)
+         (map_IndexedQS_Rep Index idx (GetIndexedRelation r_o (map_IndexedQS_idx Index idx)))
+         (i2th_Bounded ADTSigname r_n idx).
+
+Definition map_IndexedQS_Rep''
+           {indices}
+           (Index : ilist (fun ns : NamedSchema => SearchUpdateTerms (schemaHeading (relSchema ns))) indices )
+           idx
+           (rep : @IndexedEnsemble
+                    (@Tuple
+                       (schemaHeading
+                          (relSchema
+                             (@nth_Bounded NamedSchema string relName
+                                           indices idx)))))
+: Rep
+    (ith_Bounded ADTSigname
+                 (Build_IndexedQueryStructure_Impl_Specs Index) (map_IndexedQS_idx' Index idx)).
+Proof.
+  destruct idx as [idx [n nth_n]].
+  revert Index idx n nth_n rep.
+  induction indices; destruct n; simpl; intros; try discriminate; eauto.
+  eapply IHindices; eauto.
+Defined.
+
+Definition Build_IndexedQueryStructure_Impl_AbsR''
+           {qs_schema : QueryStructureSchema}
+           (Index : ilist (fun ns : NamedSchema => SearchUpdateTerms (schemaHeading (relSchema ns))) (qschemaSchemas qs_schema) )
+           (DelegateImpls : ilist (fun ns => cADT (namedADTSig ns))
+                                  (Build_IndexedQueryStructure_Impl_Sigs Index))
+           (ValidImpl :
+              forall idx : BoundedIndex (map relName (qschemaSchemas qs_schema)),
+                refineADT (ith_Bounded ADTSigname
+                                       (Build_IndexedQueryStructure_Impl_Specs Index) (map_IndexedQS_idx' Index idx))
+                          (LiftcADT (ith_Bounded ADTSigname _ (map_IndexedQS_idx' Index idx))))
+           (r_o : IndexedQueryStructure qs_schema Index)
+           (r_n : Build_IndexedQueryStructure_Impl_cRep Index DelegateImpls)
+: Prop :=
+  forall idx,
+    AbsR (ValidImpl idx)
+         (map_IndexedQS_Rep'' Index idx (GetIndexedRelation r_o idx))
+         (i2th_Bounded ADTSigname r_n (map_IndexedQS_idx' Index idx)).
+
+Definition CallBagImplMethod
+           {qs_schema : QueryStructureSchema}
+           (Index : ilist (fun ns : NamedSchema => SearchUpdateTerms (schemaHeading (relSchema ns))) (qschemaSchemas qs_schema) )
+           (DelegateImpls : ilist (fun ns => cADT (namedADTSig ns))
+                                  (Build_IndexedQueryStructure_Impl_Sigs Index))
+           idx midx
+           (r_n : Build_IndexedQueryStructure_Impl_cRep Index DelegateImpls) :=
+  cMethods (ith_Bounded ADTSigname _ idx) midx (i2th_Bounded _ r_n idx).
+
+Definition CallBagImplConstructor
+           {qs_schema : QueryStructureSchema}
+           (Index : ilist (fun ns : NamedSchema => SearchUpdateTerms (schemaHeading (relSchema ns))) (qschemaSchemas qs_schema) )
+           (DelegateImpls : ilist (fun ns => cADT (namedADTSig ns))
+                                  (Build_IndexedQueryStructure_Impl_Sigs Index))
+           idx midx :=
+  cConstructors (ith_Bounded ADTSigname DelegateImpls idx) midx .
+
+Fixpoint Build_IndexedQueryStructure_Impl_midx
+         {indices}
+         (P : ADTSig -> Type)
+: forall (Index : ilist (fun ns : NamedSchema => SearchUpdateTerms (schemaHeading (relSchema ns))) indices)
+         ridx
+         (midx : P
+                   (BagSig (@Tuple (schemaHeading
+                                      (relSchema
+                                         (@nth_Bounded NamedSchema string relName
+                                                       indices (map_IndexedQS_idx Index ridx ) ))))
+                           (BagSearchTermType
+                              (ith_Bounded relName Index (map_IndexedQS_idx Index ridx)))
+                           (BagUpdateTermType
+                              (ith_Bounded relName Index (map_IndexedQS_idx Index ridx))))),
+    P
+      (namedADTSig
+         (nth_Bounded ADTSigname (Build_IndexedQueryStructure_Impl_Sigs Index)
+                      ridx)) :=
+  match indices return
+        forall (Index : ilist
+                          (fun ns : NamedSchema =>
+                             SearchUpdateTerms (schemaHeading (relSchema ns)))
+                          indices)
+               (ridx : BoundedIndex
+                         (map ADTSigname (Build_IndexedQueryStructure_Impl_Sigs Index)))
+               (midx : P
+                         (BagSig (@Tuple (schemaHeading
+                                            (relSchema
+                                               (@nth_Bounded NamedSchema string relName
+                                                             indices (map_IndexedQS_idx Index ridx ) ))))
+                                 (BagSearchTermType
+                                    (ith_Bounded relName Index (map_IndexedQS_idx Index ridx)))
+                                 (BagUpdateTermType
+                                    (ith_Bounded relName Index (map_IndexedQS_idx Index ridx))))),
+          P
+            (namedADTSig
+               (nth_Bounded ADTSigname (Build_IndexedQueryStructure_Impl_Sigs Index)
+                            ridx))
+  with
+    | nil => fun _ ridx => BoundedIndex_nil _ ridx
+    | ns :: indices' =>
+      fun Index ridx =>
+        match ridx with
+          | {| bindex := ridx;
+               indexb := {|ibound := n;
+                           boundi := nth_n |}|} =>
+            match n return
+                  forall
+                    (Index' : ilist
+                                (fun ns : NamedSchema =>
+                                   SearchUpdateTerms (schemaHeading (relSchema ns))) (ns :: indices'))
+                    ridx nth_n,
+                    let idx := {| bindex := ridx;
+                                  indexb := {|ibound := n;
+                                              boundi := nth_n |}|} in
+                    P
+                      (BagSig (@Tuple (schemaHeading
+                                         (relSchema
+                                            (@nth_Bounded NamedSchema string relName
+                                                          (ns :: indices') (map_IndexedQS_idx Index' idx ) ))))
+                              (BagSearchTermType
+                                 (ith_Bounded relName Index' (map_IndexedQS_idx Index' idx)))
+                              (BagUpdateTermType
+                                 (ith_Bounded relName Index' (map_IndexedQS_idx Index' idx)))) ->
+                    P
+                      (namedADTSig
+                         (nth_Bounded ADTSigname (Build_IndexedQueryStructure_Impl_Sigs Index')
+                                      {| bindex := ridx;
+                                         indexb := {|ibound := n;
+                                                     boundi := nth_n |}|}))
+            with
+              | 0 => fun Index idx nth_n midx => midx
+              | S n' => fun Index idx nth_n midx =>
+                          (@Build_IndexedQueryStructure_Impl_midx
+                             indices' P (ilist_tl Index)
+                             {| bindex := idx;
+                                indexb := {|ibound := n';
+                                            boundi := nth_n |}|}
+                             midx)
+            end Index ridx nth_n
+        end
+  end.
+
+Definition Build_IndexedQueryStructure_Impl_MethodDom
+           {indices}
+: forall (Index : ilist (fun ns : NamedSchema => SearchUpdateTerms (schemaHeading (relSchema ns))) indices)
+         ridx
+         midx,
+    fst (MethodDomCod
+           (BagSig (@Tuple (schemaHeading (relSchema (nth_Bounded relName indices  ridx))))
+                   (BagSearchTermType
+                      (ith_Bounded relName Index ridx))
+                   (BagUpdateTermType
+                      (ith_Bounded relName Index ridx)))
+           midx)
     -> fst
-        (MethodDomCod
-           (namedADTSig
-              (nth_Bounded ADTSigname
-                           (Build_IndexedQueryStructure_Impl_Sigs Index) (map_IndexedQS_idx' Index ridx)))
-           (Build_IndexedQueryStructure_Impl_midx MethodIndex Index (map_IndexedQS_idx' Index ridx) midx)).
-  Proof.
-    destruct ridx as [idx [n nth_n]]; revert Index idx n nth_n.
-    induction indices.
+         (MethodDomCod
+            (namedADTSig
+               (nth_Bounded ADTSigname
+                            (Build_IndexedQueryStructure_Impl_Sigs Index) (map_IndexedQS_idx' Index ridx)))
+            (Build_IndexedQueryStructure_Impl_midx MethodIndex Index (map_IndexedQS_idx' Index ridx) midx)).
+Proof.
+  destruct ridx as [idx [n nth_n]]; revert Index idx n nth_n.
+  induction indices.
   - destruct n; simpl; discriminate.
   - destruct n; simpl; eauto.
     intros; eapply (IHindices (ilist_tl Index) idx n nth_n); eauto.
-  Defined.
+Defined.
 
-  Definition Build_IndexedQueryStructure_Impl_MethodCod
+Definition Build_IndexedQueryStructure_Impl_MethodCod
            {indices}
-  : forall (Index : ilist (fun ns : NamedSchema => SearchUpdateTerms (schemaHeading (relSchema ns))) indices)
-           ridx
-           midx,
-      snd
-        (MethodDomCod
-           (namedADTSig
-              (nth_Bounded ADTSigname
-                           (Build_IndexedQueryStructure_Impl_Sigs Index) (map_IndexedQS_idx' Index ridx)))
-           (Build_IndexedQueryStructure_Impl_midx MethodIndex Index (map_IndexedQS_idx' Index ridx) midx))
-  ->       snd (MethodDomCod
-             (BagSig (@Tuple (schemaHeading (relSchema (nth_Bounded relName indices  ridx))))
-                     (BagSearchTermType
-                        (ith_Bounded relName Index ridx))
-                     (BagUpdateTermType
-                        (ith_Bounded relName Index ridx)))
-             midx)
+: forall (Index : ilist (fun ns : NamedSchema => SearchUpdateTerms (schemaHeading (relSchema ns))) indices)
+         ridx
+         midx,
+    snd
+      (MethodDomCod
+         (namedADTSig
+            (nth_Bounded ADTSigname
+                         (Build_IndexedQueryStructure_Impl_Sigs Index) (map_IndexedQS_idx' Index ridx)))
+         (Build_IndexedQueryStructure_Impl_midx MethodIndex Index (map_IndexedQS_idx' Index ridx) midx))
+    ->       snd (MethodDomCod
+                    (BagSig (@Tuple (schemaHeading (relSchema (nth_Bounded relName indices  ridx))))
+                            (BagSearchTermType
+                               (ith_Bounded relName Index ridx))
+                            (BagUpdateTermType
+                               (ith_Bounded relName Index ridx)))
+                    midx)
 .
-  Proof.
-    destruct ridx as [idx [n nth_n]]; revert Index idx n nth_n.
-    induction indices.
+Proof.
+  destruct ridx as [idx [n nth_n]]; revert Index idx n nth_n.
+  induction indices.
   - destruct n; simpl; discriminate.
   - destruct n; simpl; eauto.
     intros; eapply (IHindices (ilist_tl Index) idx n nth_n); eauto.
-  Defined.
+Defined.
 
 Lemma ith_Build_IndexedQueryStructure_Impl_Methods
-        {indices}
-  : forall
-      (Index : ilist (fun ns : NamedSchema => SearchUpdateTerms (schemaHeading (relSchema ns))) indices )
-      (idx : BoundedIndex
-               (map ADTSigname
-                    (Build_IndexedQueryStructure_Impl_Sigs Index))),
-      Methods (ith_Bounded ADTSigname (Build_IndexedQueryStructure_Impl_Specs Index) idx) =
-      eq_rect _ (fun r => forall idx, methodType (Rep r) _ _ )
-              (Methods (eq_rect _ ADT
-                                (@BagSpec (@Tuple (schemaHeading (relSchema (@nth_Bounded NamedSchema string relName
-                                                                                          indices (map_IndexedQS_idx Index idx)))))
-                                          (BagSearchTermType (ith_Bounded _ Index (map_IndexedQS_idx Index idx)))
-                                          (BagUpdateTermType (ith_Bounded _ Index (map_IndexedQS_idx Index idx)))
-                                          (BagMatchSearchTerm (ith_Bounded _ Index (map_IndexedQS_idx Index idx)))
-                                          (BagApplyUpdateTerm (ith_Bounded _ Index (map_IndexedQS_idx Index idx))))
-                                _ (ith_Build_IndexedQueryStructure_Impl_Sigs_eq Index idx)))
-              _ (eq_sym (ith_Build_IndexedQueryStructure_Impl_Specs_eq Index idx)).
-  Proof.
-    destruct idx as [idx [n nth_n]].
-    revert Index idx n nth_n.
-    induction indices; destruct n; simpl; intros; try discriminate; eauto.
-    eapply (IHindices (ilist_tl Index) idx n nth_n).
-  Defined.
+      {indices}
+: forall
+    (Index : ilist (fun ns : NamedSchema => SearchUpdateTerms (schemaHeading (relSchema ns))) indices )
+    (idx : BoundedIndex
+             (map ADTSigname
+                  (Build_IndexedQueryStructure_Impl_Sigs Index))),
+    Methods (ith_Bounded ADTSigname (Build_IndexedQueryStructure_Impl_Specs Index) idx) =
+    eq_rect _ (fun r => forall idx, methodType (Rep r) _ _ )
+            (Methods (eq_rect _ ADT
+                              (@BagSpec (@Tuple (schemaHeading (relSchema (@nth_Bounded NamedSchema string relName
+                                                                                        indices (map_IndexedQS_idx Index idx)))))
+                                        (BagSearchTermType (ith_Bounded _ Index (map_IndexedQS_idx Index idx)))
+                                        (BagUpdateTermType (ith_Bounded _ Index (map_IndexedQS_idx Index idx)))
+                                        (BagMatchSearchTerm (ith_Bounded _ Index (map_IndexedQS_idx Index idx)))
+                                        (BagApplyUpdateTerm (ith_Bounded _ Index (map_IndexedQS_idx Index idx))))
+                              _ (ith_Build_IndexedQueryStructure_Impl_Sigs_eq Index idx)))
+            _ (eq_sym (ith_Build_IndexedQueryStructure_Impl_Specs_eq Index idx)).
+Proof.
+  destruct idx as [idx [n nth_n]].
+  revert Index idx n nth_n.
+  induction indices; destruct n; simpl; intros; try discriminate; eauto.
+  eapply (IHindices (ilist_tl Index) idx n nth_n).
+Defined.
 
-  Lemma refine_Mapped_Methods
-        {indices}
-        (Index : ilist (fun ns : NamedSchema => SearchUpdateTerms (schemaHeading (relSchema ns))) (indices) )
-  :  forall
-      ridx,
-      forall
-        (r_o : @IndexedEnsemble (@Tuple (schemaHeading (relSchema (nth_Bounded relName indices ridx)))))
-      midx
-      d r s,
-        let ridx' := map_IndexedQS_idx' Index ridx in
-        let midx' := Build_IndexedQueryStructure_Impl_midx MethodIndex Index ridx' midx in
-        let d' := Build_IndexedQueryStructure_Impl_MethodDom Index ridx _ d in
-Methods
-     (ith_Bounded ADTSigname (Build_IndexedQueryStructure_Impl_Specs Index) ridx') midx'
-     (map_IndexedQS_Rep'' Index ridx r_o) d'
-     ↝ (r, s) ->
-Methods
-  (BagSpec (BagMatchSearchTerm (ith_Bounded relName Index ridx))
-           (BagApplyUpdateTerm (ith_Bounded relName Index ridx))) midx r_o d
-   ↝ (map_IndexedQS_Rep' Index ridx r,
-     Build_IndexedQueryStructure_Impl_MethodCod Index ridx midx s).
-  Proof.
-    intros; pose proof (ith_Build_IndexedQueryStructure_Impl_Methods Index ridx') as H';
-    rewrite H' in H; revert H; clear H'.
-    unfold d', midx', ridx' in *; clear ridx' midx' d'.
-    revert r_o d r s.
-    intro; eapply (Iterate_Dep_Type_BoundedIndex_equiv_1) with (idx := midx);
-    simpl.
-    intuition;
-      simpl in *;
-      first [revert midx r_o d r s H
-            | revert midx r_o b a r s H ];
+Lemma refine_Mapped_Methods
+      {indices}
+      (Index : ilist (fun ns : NamedSchema => SearchUpdateTerms (schemaHeading (relSchema ns))) (indices) )
+:  forall
+    ridx,
+  forall
+    (r_o : @IndexedEnsemble (@Tuple (schemaHeading (relSchema (nth_Bounded relName indices ridx)))))
+    midx
+    d r s,
+    let ridx' := map_IndexedQS_idx' Index ridx in
+    let midx' := Build_IndexedQueryStructure_Impl_midx MethodIndex Index ridx' midx in
+    let d' := Build_IndexedQueryStructure_Impl_MethodDom Index ridx _ d in
+    Methods
+      (ith_Bounded ADTSigname (Build_IndexedQueryStructure_Impl_Specs Index) ridx') midx'
+      (map_IndexedQS_Rep'' Index ridx r_o) d'
+      ↝ (r, s) ->
+    Methods
+      (BagSpec (BagMatchSearchTerm (ith_Bounded relName Index ridx))
+               (BagApplyUpdateTerm (ith_Bounded relName Index ridx))) midx r_o d
+      ↝ (map_IndexedQS_Rep' Index ridx r,
+         Build_IndexedQueryStructure_Impl_MethodCod Index ridx midx s).
+Proof.
+  intros; pose proof (ith_Build_IndexedQueryStructure_Impl_Methods Index ridx') as H';
+  rewrite H' in H; revert H; clear H'.
+  unfold d', midx', ridx' in *; clear ridx' midx' d'.
+  revert r_o d r s.
+  intro; eapply (Iterate_Dep_Type_BoundedIndex_equiv_1) with (idx := midx);
+  simpl.
+  intuition;
+    simpl in *;
+    first [revert midx r_o d r s H
+          | revert midx r_o b a r s H ];
     try (destruct ridx as [idx [n nth_n]];
-      revert idx n nth_n;
-      unfold IndexedQueryStructure, GetIndexedRelation in *;
-      unfold list_ind, list_rect in *;
-      induction indices; destruct n; simpl; try (intros; discriminate); eauto;
-      eapply IHindices).
-  Qed.
+         revert idx n nth_n;
+         unfold IndexedQueryStructure, GetIndexedRelation in *;
+           unfold list_ind, list_rect in *;
+           induction indices; destruct n; simpl; try (intros; discriminate); eauto;
+         eapply IHindices).
+Qed.
 
-  Lemma map_indexedqs_Rep'_id
-        {indices}
-  : forall Index idx r_o,
-      map_IndexedQS_Rep'' (indices := indices) Index idx (map_IndexedQS_Rep' Index idx r_o) = r_o.
-  Proof.
-    destruct idx as [idx [n nth_n]]; revert Index idx n nth_n.
-    induction indices; simpl; intros.
-    - destruct n; discriminate.
-    - destruct n; simpl in *; eauto.
-      eapply (IHindices (ilist_tl Index)).
-  Qed.
+Lemma map_indexedqs_Rep'_id
+      {indices}
+: forall Index idx r_o,
+    map_IndexedQS_Rep'' (indices := indices) Index idx (map_IndexedQS_Rep' Index idx r_o) = r_o.
+Proof.
+  destruct idx as [idx [n nth_n]]; revert Index idx n nth_n.
+  induction indices; simpl; intros.
+  - destruct n; discriminate.
+  - destruct n; simpl in *; eauto.
+    eapply (IHindices (ilist_tl Index)).
+Qed.
 
-  Lemma Update_Build_IndexedQueryStructure_Impl_AbsR''
-        {qs_schema}
-        Index
-  : forall
-      DelegateImpl
+Lemma Update_Build_IndexedQueryStructure_Impl_AbsR''
+      {qs_schema}
+      Index
+: forall
+    DelegateImpl
+    ValidImpl
+    (r_o : IndexedQueryStructure qs_schema Index)
+    (r_n : Build_IndexedQueryStructure_Impl_cRep Index DelegateImpl)
+    idx r_o' r_n',
+    Build_IndexedQueryStructure_Impl_AbsR'' ValidImpl r_o r_n
+    -> AbsR (ValidImpl idx) r_o' r_n'
+    -> Build_IndexedQueryStructure_Impl_AbsR''
+         ValidImpl
+         (UpdateIndexedRelation r_o idx (map_IndexedQS_Rep' _ _ r_o'))
+         (replace_BoundedIndex2 _ r_n (map_IndexedQS_idx' _ idx) r_n').
+Proof.
+  intros; intro idx'.
+  destruct (BoundedString_eq_dec idx idx'); subst.
+  - rewrite i2th_replace_BoundIndex_eq, get_update_indexed_eq, map_indexedqs_Rep'_id; eauto.
+  - rewrite i2th_replace_BoundIndex_neq, get_update_indexed_neq; eauto using string_dec.
+    intuition; apply n.
+    destruct idx as [idx [m nth_m]]; destruct idx' as [idx' [n' nth_n']]; simpl in *.
+    injection H1; intros; subst; repeat f_equal.
+    unfold map_IndexedQS_idx' in H1; simpl in H1.
+    apply eq_proofs_unicity_Opt_A; eauto using string_dec.
+Qed.
+
+Lemma refine_BagImplMethods'
+      {qs_schema : QueryStructureSchema}
+      (Index : ilist (fun ns : NamedSchema => SearchUpdateTerms (schemaHeading (relSchema ns))) (qschemaSchemas qs_schema) )
+      (DelegateImpls : ilist (fun ns => cADT (namedADTSig ns))
+                             (Build_IndexedQueryStructure_Impl_Sigs Index))
       ValidImpl
-      (r_o : IndexedQueryStructure qs_schema Index)
-      (r_n : Build_IndexedQueryStructure_Impl_cRep Index DelegateImpl)
-      idx r_o' r_n',
-      Build_IndexedQueryStructure_Impl_AbsR'' ValidImpl r_o r_n
-      -> AbsR (ValidImpl idx) r_o' r_n'
-      -> Build_IndexedQueryStructure_Impl_AbsR''
-           ValidImpl
-           (UpdateIndexedRelation r_o idx (map_IndexedQS_Rep' _ _ r_o'))
-           (replace_BoundedIndex2 _ r_n (map_IndexedQS_idx' _ idx) r_n').
-  Proof.
-    intros; intro idx'.
-    destruct (BoundedString_eq_dec idx idx'); subst.
-    - rewrite i2th_replace_BoundIndex_eq, get_update_indexed_eq, map_indexedqs_Rep'_id; eauto.
-    - rewrite i2th_replace_BoundIndex_neq, get_update_indexed_neq; eauto using string_dec.
-      intuition; apply n.
-      destruct idx as [idx [m nth_m]]; destruct idx' as [idx' [n' nth_n']]; simpl in *.
-      injection H1; intros; subst; repeat f_equal.
-      unfold map_IndexedQS_idx' in H1; simpl in H1.
-      apply eq_proofs_unicity_Opt_A; eauto using string_dec.
-  Qed.
-
-  Lemma refine_BagImplMethods'
-        {qs_schema : QueryStructureSchema}
-        (Index : ilist (fun ns : NamedSchema => SearchUpdateTerms (schemaHeading (relSchema ns))) (qschemaSchemas qs_schema) )
-        (DelegateImpls : ilist (fun ns => cADT (namedADTSig ns))
-                               (Build_IndexedQueryStructure_Impl_Sigs Index))
-        ValidImpl
-  :  forall (r_o : IndexedQueryStructure qs_schema Index)
-            (r_n : Build_IndexedQueryStructure_Impl_cRep Index DelegateImpls)
-            ridx,
-       let ridx' := map_IndexedQS_idx' Index ridx in
-       Build_IndexedQueryStructure_Impl_AbsR'' ValidImpl r_o r_n ->
-            forall (midx : MethodIndex
-                     (BagSig Tuple
-                             (BagSearchTermType
-                                (ith_Bounded relName Index (map_IndexedQS_idx Index ridx')))
-                             (BagUpdateTermType
-                                (ith_Bounded relName Index (map_IndexedQS_idx Index ridx')))))
-                   (d : fst
-                          (MethodDomCod
-                             (BagSig (@Tuple (schemaHeading (relSchema (nth_Bounded relName (qschemaSchemas qs_schema) ridx))))
-                                     (BagSearchTermType (ith_Bounded relName Index ridx))
-                                     (BagUpdateTermType (ith_Bounded relName Index ridx))) midx)),
+:  forall (r_o : IndexedQueryStructure qs_schema Index)
+          (r_n : Build_IndexedQueryStructure_Impl_cRep Index DelegateImpls)
+          ridx,
+     let ridx' := map_IndexedQS_idx' Index ridx in
+     Build_IndexedQueryStructure_Impl_AbsR'' ValidImpl r_o r_n ->
+     forall (midx : MethodIndex
+                      (BagSig Tuple
+                              (BagSearchTermType
+                                 (ith_Bounded relName Index (map_IndexedQS_idx Index ridx')))
+                              (BagUpdateTermType
+                                 (ith_Bounded relName Index (map_IndexedQS_idx Index ridx')))))
+            (d : fst
+                   (MethodDomCod
+                      (BagSig (@Tuple (schemaHeading (relSchema (nth_Bounded relName (qschemaSchemas qs_schema) ridx))))
+                              (BagSearchTermType (ith_Bounded relName Index ridx))
+                              (BagUpdateTermType (ith_Bounded relName Index ridx))) midx)),
        let midx' := Build_IndexedQueryStructure_Impl_midx MethodIndex Index ridx' midx in
        let d' := Build_IndexedQueryStructure_Impl_MethodDom Index ridx _ d in
        exists r_o',
-                  refine (CallBagMethod ridx midx r_o d)
-                  (ret (map_IndexedQS_Rep' _ _ r_o',
-                        Build_IndexedQueryStructure_Impl_MethodCod Index ridx _
-                                                                   (snd (CallBagImplMethod (map_IndexedQS_idx' Index ridx) midx' r_n d'))))
-                  /\ AbsR (ValidImpl ridx) r_o' (fst (CallBagImplMethod ridx' midx' r_n d')).
-  Proof.
-    intros.
-    pose proof (ADTRefinementPreservesMethods (ValidImpl ridx) midx'
-                                              (map_IndexedQS_Rep'' Index ridx
+         refine (CallBagMethod ridx midx r_o d)
+                (ret (map_IndexedQS_Rep' _ _ r_o',
+                      Build_IndexedQueryStructure_Impl_MethodCod Index ridx _
+                                                                 (snd (CallBagImplMethod (map_IndexedQS_idx' Index ridx) midx' r_n d'))))
+         /\ AbsR (ValidImpl ridx) r_o' (fst (CallBagImplMethod ridx' midx' r_n d')).
+Proof.
+  intros.
+  pose proof (ADTRefinementPreservesMethods (ValidImpl ridx) midx'
+                                            (map_IndexedQS_Rep'' Index ridx
                                                                  (GetIndexedRelation r_o ridx))
-                                              (i2th_Bounded _ r_n ridx') d' (H ridx) (ReturnComputes _)).
-    Local Arguments map_IndexedQS_Rep : simpl never.
-    inversion_by computes_to_inv; subst.
-    exists (fst x);
-      unfold CallBagImplMethod; simpl in *.
-      split; simpl.
-      - pose proof (f_equal snd H3) as eq_x; simpl in eq_x.
-        assert (refine (CallBagMethod ridx midx r_o d)
-                       (ret
-                          (map_IndexedQS_Rep' Index ridx (fst x),
-                           Build_IndexedQueryStructure_Impl_MethodCod Index ridx midx (snd x))));
-          [ | rewrite eq_x in H0;  eapply H0 ].
-        intros v Comp_v; simpl in *; inversion_by computes_to_inv; subst.
-        destruct x; simpl @fst in *; simpl @snd in *.
-        unfold ridx' in *.
-        revert H1.
-        Local Transparent CallBagMethod.
-        eapply refine_Mapped_Methods.
-      - pose proof (f_equal fst H3) as eq_x0; simpl in eq_x0.
-        rewrite eq_x0 in H2; simpl in H2; apply H2.
-  Qed.
+                                            (i2th_Bounded _ r_n ridx') d' (H ridx) (ReturnComputes _)).
+  Local Arguments map_IndexedQS_Rep : simpl never.
+  inversion_by computes_to_inv; subst.
+  exists (fst x);
+    unfold CallBagImplMethod; simpl in *.
+  split; simpl.
+  - pose proof (f_equal snd H3) as eq_x; simpl in eq_x.
+    assert (refine (CallBagMethod ridx midx r_o d)
+                   (ret
+                      (map_IndexedQS_Rep' Index ridx (fst x),
+                       Build_IndexedQueryStructure_Impl_MethodCod Index ridx midx (snd x))));
+      [ | rewrite eq_x in H0;  eapply H0 ].
+    intros v Comp_v; simpl in *; inversion_by computes_to_inv; subst.
+    destruct x; simpl @fst in *; simpl @snd in *.
+    unfold ridx' in *.
+    revert H1.
+    Local Transparent CallBagMethod.
+    eapply refine_Mapped_Methods.
+  - pose proof (f_equal fst H3) as eq_x0; simpl in eq_x0.
+    rewrite eq_x0 in H2; simpl in H2; apply H2.
+Qed.
 
-  Lemma refine_BagImplMethods
-        {qs_schema : QueryStructureSchema}
-        (Index : ilist (fun ns : NamedSchema => SearchUpdateTerms (schemaHeading (relSchema ns))) (qschemaSchemas qs_schema) )
-        (DelegateImpls : ilist (fun ns => cADT (namedADTSig ns))
-                               (Build_IndexedQueryStructure_Impl_Sigs Index))
-        ValidImpl
-  :  forall (r_o : IndexedQueryStructure qs_schema Index)
-            (r_n : Build_IndexedQueryStructure_Impl_cRep Index DelegateImpls)
-            ridx,
-       let ridx' := map_IndexedQS_idx' Index ridx in
-       Build_IndexedQueryStructure_Impl_AbsR'' ValidImpl r_o r_n ->
-            forall (midx : MethodIndex
-                     (BagSig Tuple
-                             (BagSearchTermType
-                                (ith_Bounded relName Index (map_IndexedQS_idx Index ridx')))
-                             (BagUpdateTermType
-                                (ith_Bounded relName Index (map_IndexedQS_idx Index ridx')))))
-                   (d : fst
-                          (MethodDomCod
-                             (BagSig (@Tuple (schemaHeading (relSchema (nth_Bounded relName (qschemaSchemas qs_schema) ridx))))
-                                     (BagSearchTermType (ith_Bounded relName Index ridx))
-                                     (BagUpdateTermType (ith_Bounded relName Index ridx))) midx)),
+Lemma refine_BagImplMethods
+      {qs_schema : QueryStructureSchema}
+      (Index : ilist (fun ns : NamedSchema => SearchUpdateTerms (schemaHeading (relSchema ns))) (qschemaSchemas qs_schema) )
+      (DelegateImpls : ilist (fun ns => cADT (namedADTSig ns))
+                             (Build_IndexedQueryStructure_Impl_Sigs Index))
+      ValidImpl
+:  forall (r_o : IndexedQueryStructure qs_schema Index)
+          (r_n : Build_IndexedQueryStructure_Impl_cRep Index DelegateImpls)
+          ridx,
+     let ridx' := map_IndexedQS_idx' Index ridx in
+     Build_IndexedQueryStructure_Impl_AbsR'' ValidImpl r_o r_n ->
+     forall (midx : MethodIndex
+                      (BagSig Tuple
+                              (BagSearchTermType
+                                 (ith_Bounded relName Index (map_IndexedQS_idx Index ridx')))
+                              (BagUpdateTermType
+                                 (ith_Bounded relName Index (map_IndexedQS_idx Index ridx')))))
+            (d : fst
+                   (MethodDomCod
+                      (BagSig (@Tuple (schemaHeading (relSchema (nth_Bounded relName (qschemaSchemas qs_schema) ridx))))
+                              (BagSearchTermType (ith_Bounded relName Index ridx))
+                              (BagUpdateTermType (ith_Bounded relName Index ridx))) midx)),
        let midx' := Build_IndexedQueryStructure_Impl_midx MethodIndex Index ridx' midx in
        let d' := Build_IndexedQueryStructure_Impl_MethodDom Index ridx _ d in
        exists r_o',
-                  refine (CallBagMethod ridx midx r_o d)
-                  (ret (map_IndexedQS_Rep' Index _ r_o',
-                        Build_IndexedQueryStructure_Impl_MethodCod Index ridx _
-                                                                   (snd (CallBagImplMethod (map_IndexedQS_idx' Index ridx) midx' r_n d'))))
-                  /\ Build_IndexedQueryStructure_Impl_AbsR''
-                       ValidImpl
-                       (UpdateIndexedRelation r_o ridx (map_IndexedQS_Rep' _ _ r_o'))
-                       (replace_BoundedIndex2 _ r_n ridx' (fst (CallBagImplMethod ridx' midx' r_n d'))) .
-  Proof.
-    intros; destruct (@refine_BagImplMethods' _ Index DelegateImpls ValidImpl r_o r_n ridx H midx d)
-                     as [r_o' [refines_r_o' AbsR_r_o']].
-    exists r_o'; split; eauto.
-    eauto using Update_Build_IndexedQueryStructure_Impl_AbsR''.
-  Qed.
+         refine (CallBagMethod ridx midx r_o d)
+                (ret (map_IndexedQS_Rep' Index _ r_o',
+                      Build_IndexedQueryStructure_Impl_MethodCod Index ridx _
+                                                                 (snd (CallBagImplMethod (map_IndexedQS_idx' Index ridx) midx' r_n d'))))
+         /\ Build_IndexedQueryStructure_Impl_AbsR''
+              ValidImpl
+              (UpdateIndexedRelation r_o ridx (map_IndexedQS_Rep' _ _ r_o'))
+              (replace_BoundedIndex2 _ r_n ridx' (fst (CallBagImplMethod ridx' midx' r_n d'))) .
+Proof.
+  intros; destruct (@refine_BagImplMethods' _ Index DelegateImpls ValidImpl r_o r_n ridx H midx d)
+    as [r_o' [refines_r_o' AbsR_r_o']].
+  exists r_o'; split; eauto.
+  eauto using Update_Build_IndexedQueryStructure_Impl_AbsR''.
+Qed.
 
-  Definition Build_IndexedQueryStructure_Impl_ConstructorDom
+Definition Build_IndexedQueryStructure_Impl_ConstructorDom
            {indices}
-  : forall (Index : ilist (fun ns : NamedSchema => SearchUpdateTerms (schemaHeading (relSchema ns))) indices)
-           ridx
-           cidx,
-      ConstructorDom
-             (BagSig (@Tuple (schemaHeading (relSchema (nth_Bounded relName indices  ridx))))
-                     (BagSearchTermType
-                        (ith_Bounded relName Index ridx))
-                     (BagUpdateTermType
-                        (ith_Bounded relName Index ridx)))
-             cidx
-      ->       ConstructorDom
-        (namedADTSig
-           (nth_Bounded ADTSigname
-                        (Build_IndexedQueryStructure_Impl_Sigs Index) (map_IndexedQS_idx' Index ridx)))
-        (Build_IndexedQueryStructure_Impl_midx ConstructorIndex Index (map_IndexedQS_idx' Index ridx) cidx).
-  Proof.
-    destruct ridx as [idx [n nth_n]]; revert Index idx n nth_n.
-    induction indices.
+: forall (Index : ilist (fun ns : NamedSchema => SearchUpdateTerms (schemaHeading (relSchema ns))) indices)
+         ridx
+         cidx,
+    ConstructorDom
+      (BagSig (@Tuple (schemaHeading (relSchema (nth_Bounded relName indices  ridx))))
+              (BagSearchTermType
+                 (ith_Bounded relName Index ridx))
+              (BagUpdateTermType
+                 (ith_Bounded relName Index ridx)))
+      cidx
+    ->       ConstructorDom
+               (namedADTSig
+                  (nth_Bounded ADTSigname
+                               (Build_IndexedQueryStructure_Impl_Sigs Index) (map_IndexedQS_idx' Index ridx)))
+               (Build_IndexedQueryStructure_Impl_midx ConstructorIndex Index (map_IndexedQS_idx' Index ridx) cidx).
+Proof.
+  destruct ridx as [idx [n nth_n]]; revert Index idx n nth_n.
+  induction indices.
   - destruct n; simpl; discriminate.
   - destruct n; simpl; eauto.
     intros; eapply (IHindices (ilist_tl Index) idx n nth_n); eauto.
-  Defined.
+Defined.
 
 Lemma ith_Build_IndexedQueryStructure_Impl_Constructors
-        {indices}
-  : forall
-      (Index : ilist (fun ns : NamedSchema => SearchUpdateTerms (schemaHeading (relSchema ns))) indices )
-      (idx : BoundedIndex
-               (map ADTSigname
-                    (Build_IndexedQueryStructure_Impl_Sigs Index))),
-      Constructors (ith_Bounded ADTSigname (Build_IndexedQueryStructure_Impl_Specs Index) idx) =
-      eq_rect _ (fun r => forall idx, constructorType (Rep r) _ )
-              (Constructors (eq_rect _ ADT
-                                (@BagSpec (@Tuple (schemaHeading (relSchema (@nth_Bounded NamedSchema string relName
-                                                                                          indices (map_IndexedQS_idx Index idx)))))
-                                          (BagSearchTermType (ith_Bounded _ Index (map_IndexedQS_idx Index idx)))
-                                          (BagUpdateTermType (ith_Bounded _ Index (map_IndexedQS_idx Index idx)))
-                                          (BagMatchSearchTerm (ith_Bounded _ Index (map_IndexedQS_idx Index idx)))
-                                          (BagApplyUpdateTerm (ith_Bounded _ Index (map_IndexedQS_idx Index idx))))
-                                _ (ith_Build_IndexedQueryStructure_Impl_Sigs_eq Index idx)))
-              _ (eq_sym (ith_Build_IndexedQueryStructure_Impl_Specs_eq Index idx)).
-  Proof.
-    destruct idx as [idx [n nth_n]].
-    revert Index idx n nth_n.
-    induction indices; destruct n; simpl; intros; try discriminate; eauto.
-    eapply (IHindices (ilist_tl Index) idx n nth_n).
-  Defined.
+      {indices}
+: forall
+    (Index : ilist (fun ns : NamedSchema => SearchUpdateTerms (schemaHeading (relSchema ns))) indices )
+    (idx : BoundedIndex
+             (map ADTSigname
+                  (Build_IndexedQueryStructure_Impl_Sigs Index))),
+    Constructors (ith_Bounded ADTSigname (Build_IndexedQueryStructure_Impl_Specs Index) idx) =
+    eq_rect _ (fun r => forall idx, constructorType (Rep r) _ )
+            (Constructors (eq_rect _ ADT
+                                   (@BagSpec (@Tuple (schemaHeading (relSchema (@nth_Bounded NamedSchema string relName
+                                                                                             indices (map_IndexedQS_idx Index idx)))))
+                                             (BagSearchTermType (ith_Bounded _ Index (map_IndexedQS_idx Index idx)))
+                                             (BagUpdateTermType (ith_Bounded _ Index (map_IndexedQS_idx Index idx)))
+                                             (BagMatchSearchTerm (ith_Bounded _ Index (map_IndexedQS_idx Index idx)))
+                                             (BagApplyUpdateTerm (ith_Bounded _ Index (map_IndexedQS_idx Index idx))))
+                                   _ (ith_Build_IndexedQueryStructure_Impl_Sigs_eq Index idx)))
+            _ (eq_sym (ith_Build_IndexedQueryStructure_Impl_Specs_eq Index idx)).
+Proof.
+  destruct idx as [idx [n nth_n]].
+  revert Index idx n nth_n.
+  induction indices; destruct n; simpl; intros; try discriminate; eauto.
+  eapply (IHindices (ilist_tl Index) idx n nth_n).
+Defined.
 
-  Lemma refine_Mapped_Constructor
-        {indices}
-        (Index : ilist (fun ns : NamedSchema => SearchUpdateTerms (schemaHeading (relSchema ns))) (indices) )
-  :  forall
-      ridx cidx d r,
-        let ridx' := map_IndexedQS_idx' Index ridx in
-        let cidx' := Build_IndexedQueryStructure_Impl_midx ConstructorIndex Index ridx' cidx in
-        let d' := Build_IndexedQueryStructure_Impl_ConstructorDom Index ridx _ d in
-        Constructors
-          (ith_Bounded ADTSigname (Build_IndexedQueryStructure_Impl_Specs Index) ridx') cidx' d' ↝ r ->
-Constructors
-  (BagSpec (BagMatchSearchTerm (ith_Bounded relName Index ridx))
-           (BagApplyUpdateTerm (ith_Bounded relName Index ridx))) cidx d
-   ↝ map_IndexedQS_Rep' Index ridx r.
-  Proof.
-    intros; pose proof (ith_Build_IndexedQueryStructure_Impl_Constructors Index ridx') as H';
-    rewrite H' in H; revert H; clear H'.
-    unfold d', cidx', ridx' in *; clear ridx' cidx' d'.
-    revert d r.
-    eapply (fun P H => Iterate_Dep_Type_BoundedIndex_equiv_1 P H cidx).
-    simpl.
-    intuition;
-      simpl in *;
-      first [revert cidx d r H
-            | revert cidx b a r H ];
+Lemma refine_Mapped_Constructor
+      {indices}
+      (Index : ilist (fun ns : NamedSchema => SearchUpdateTerms (schemaHeading (relSchema ns))) (indices) )
+:  forall
+    ridx cidx d r,
+    let ridx' := map_IndexedQS_idx' Index ridx in
+    let cidx' := Build_IndexedQueryStructure_Impl_midx ConstructorIndex Index ridx' cidx in
+    let d' := Build_IndexedQueryStructure_Impl_ConstructorDom Index ridx _ d in
+    Constructors
+      (ith_Bounded ADTSigname (Build_IndexedQueryStructure_Impl_Specs Index) ridx') cidx' d' ↝ r ->
+    Constructors
+      (BagSpec (BagMatchSearchTerm (ith_Bounded relName Index ridx))
+               (BagApplyUpdateTerm (ith_Bounded relName Index ridx))) cidx d
+      ↝ map_IndexedQS_Rep' Index ridx r.
+Proof.
+  intros; pose proof (ith_Build_IndexedQueryStructure_Impl_Constructors Index ridx') as H';
+  rewrite H' in H; revert H; clear H'.
+  unfold d', cidx', ridx' in *; clear ridx' cidx' d'.
+  revert d r.
+  eapply (fun P H => Iterate_Dep_Type_BoundedIndex_equiv_1 P H cidx).
+  simpl.
+  intuition;
+    simpl in *;
+    first [revert cidx d r H
+          | revert cidx b a r H ];
     try (destruct ridx as [idx [n nth_n]];
-      revert idx n nth_n;
-      unfold IndexedQueryStructure, GetIndexedRelation in *;
-      unfold list_ind, list_rect in *;
-      induction indices; destruct n; simpl; try (intros; discriminate); eauto;
-      eapply IHindices).
-  Qed.
+         revert idx n nth_n;
+         unfold IndexedQueryStructure, GetIndexedRelation in *;
+           unfold list_ind, list_rect in *;
+           induction indices; destruct n; simpl; try (intros; discriminate); eauto;
+         eapply IHindices).
+Qed.
 
-  Lemma refine_BagImplConstructor
-        {qs_schema : QueryStructureSchema}
-        (Index : ilist (fun ns : NamedSchema => SearchUpdateTerms (schemaHeading (relSchema ns))) (qschemaSchemas qs_schema) )
-        (DelegateImpls : ilist (fun ns => cADT (namedADTSig ns))
-                               (Build_IndexedQueryStructure_Impl_Sigs Index))
-        (ValidImpl : forall
-                        idx : BoundedIndex
-                                (map relName (qschemaSchemas qs_schema)),
-                      refineADT
-                        (ith_Bounded ADTSigname
-                           (Build_IndexedQueryStructure_Impl_Specs Index)
-                           (map_IndexedQS_idx' Index idx))
-                        (LiftcADT
-                           (ith_Bounded ADTSigname DelegateImpls
-                              (map_IndexedQS_idx' Index idx))))
-  :  forall (ridx : BoundedIndex (map relName (qschemaSchemas qs_schema))),
-       let ridx' := map_IndexedQS_idx' Index ridx in
-       forall (cidx : ConstructorIndex
-                        (BagSig Tuple
-                                (BagSearchTermType
-                                (ith_Bounded relName Index (map_IndexedQS_idx Index ridx')))
-                             (BagUpdateTermType
-                                (ith_Bounded relName Index (map_IndexedQS_idx Index ridx')))))
-                   (d : ConstructorDom
-                             (BagSig (@Tuple (schemaHeading (relSchema (nth_Bounded relName (qschemaSchemas qs_schema) ridx))))
-                                     (BagSearchTermType (ith_Bounded relName Index ridx))
-                                     (BagUpdateTermType (ith_Bounded relName Index ridx))) cidx),
+Lemma refine_BagImplConstructor
+      {qs_schema : QueryStructureSchema}
+      (Index : ilist (fun ns : NamedSchema => SearchUpdateTerms (schemaHeading (relSchema ns))) (qschemaSchemas qs_schema) )
+      (DelegateImpls : ilist (fun ns => cADT (namedADTSig ns))
+                             (Build_IndexedQueryStructure_Impl_Sigs Index))
+      (ValidImpl : forall
+                     idx : BoundedIndex
+                             (map relName (qschemaSchemas qs_schema)),
+                     refineADT
+                       (ith_Bounded ADTSigname
+                                    (Build_IndexedQueryStructure_Impl_Specs Index)
+                                    (map_IndexedQS_idx' Index idx))
+                       (LiftcADT
+                          (ith_Bounded ADTSigname DelegateImpls
+                                       (map_IndexedQS_idx' Index idx))))
+:  forall (ridx : BoundedIndex (map relName (qschemaSchemas qs_schema))),
+     let ridx' := map_IndexedQS_idx' Index ridx in
+     forall (cidx : ConstructorIndex
+                      (BagSig Tuple
+                              (BagSearchTermType
+                                 (ith_Bounded relName Index (map_IndexedQS_idx Index ridx')))
+                              (BagUpdateTermType
+                                 (ith_Bounded relName Index (map_IndexedQS_idx Index ridx')))))
+            (d : ConstructorDom
+                   (BagSig (@Tuple (schemaHeading (relSchema (nth_Bounded relName (qschemaSchemas qs_schema) ridx))))
+                           (BagSearchTermType (ith_Bounded relName Index ridx))
+                           (BagUpdateTermType (ith_Bounded relName Index ridx))) cidx),
        let cidx' := Build_IndexedQueryStructure_Impl_midx ConstructorIndex Index ridx' cidx in
        let d' := Build_IndexedQueryStructure_Impl_ConstructorDom Index ridx _ d in
        exists r_o' : Rep
@@ -843,39 +843,39 @@ Constructors
          refine (@CallBagConstructor _ (bindex ridx) (ith_Bounded relName Index ridx) cidx d)
                 (ret (map_IndexedQS_Rep' Index _ r_o')) /\
          AbsR (ValidImpl ridx) r_o' (CallBagImplConstructor Index DelegateImpls ridx' cidx' d').
-    Proof.
-      intros.
-      pose proof (ADTRefinementPreservesConstructors (ValidImpl ridx) cidx' d' (ReturnComputes _)).
-      Local Arguments map_IndexedQS_Rep : simpl never.
-      inversion_by computes_to_inv; subst.
-      exists x;
-        unfold CallBagImplConstructor; simpl in *.
-      split; simpl.
-      intros v Comp_v; inversion_by computes_to_inv; subst.
-      eapply refine_Mapped_Constructor; eauto.
-      eapply H1.
-    Qed.
+Proof.
+  intros.
+  pose proof (ADTRefinementPreservesConstructors (ValidImpl ridx) cidx' d' (ReturnComputes _)).
+  Local Arguments map_IndexedQS_Rep : simpl never.
+  inversion_by computes_to_inv; subst.
+  exists x;
+    unfold CallBagImplConstructor; simpl in *.
+  split; simpl.
+  intros v Comp_v; inversion_by computes_to_inv; subst.
+  eapply refine_Mapped_Constructor; eauto.
+  eapply H1.
+Qed.
 
-  Opaque CallBagConstructor.
+Opaque CallBagConstructor.
 
-  Definition Build_IndexedQueryStructure_Impl_AbsR'
-             {qs_schema : QueryStructureSchema}
-             (Index : ilist (fun ns : NamedSchema => SearchUpdateTerms (schemaHeading (relSchema ns))) (qschemaSchemas qs_schema) )
-             (DelegateImpls : ilist (fun ns => cADT (namedADTSig ns))
-                                    (Build_IndexedQueryStructure_Impl_Sigs Index))
-             (ValidImpl :
-                forall idx,
-                  refineADT (ith_Bounded ADTSigname
-                                         (Build_IndexedQueryStructure_Impl_Specs Index) idx)
-                            (LiftcADT (ith_Bounded ADTSigname DelegateImpls idx)))
-             (r_o : IndexedQueryStructure qs_schema Index)
-             (r_n : Build_IndexedQueryStructure_Impl_cRep Index DelegateImpls)
-  : Prop :=
-      @Build_IndexedQueryStructure_Impl_AbsR''
-        qs_schema Index DelegateImpls
-        (fun idx => ValidImpl (map_IndexedQS_idx' Index idx))
-        r_o
-        r_n.
+Definition Build_IndexedQueryStructure_Impl_AbsR'
+           {qs_schema : QueryStructureSchema}
+           (Index : ilist (fun ns : NamedSchema => SearchUpdateTerms (schemaHeading (relSchema ns))) (qschemaSchemas qs_schema) )
+           (DelegateImpls : ilist (fun ns => cADT (namedADTSig ns))
+                                  (Build_IndexedQueryStructure_Impl_Sigs Index))
+           (ValidImpl :
+              forall idx,
+                refineADT (ith_Bounded ADTSigname
+                                       (Build_IndexedQueryStructure_Impl_Specs Index) idx)
+                          (LiftcADT (ith_Bounded ADTSigname DelegateImpls idx)))
+           (r_o : IndexedQueryStructure qs_schema Index)
+           (r_n : Build_IndexedQueryStructure_Impl_cRep Index DelegateImpls)
+: Prop :=
+  @Build_IndexedQueryStructure_Impl_AbsR''
+    qs_schema Index DelegateImpls
+    (fun idx => ValidImpl (map_IndexedQS_idx' Index idx))
+    r_o
+    r_n.
 
 Arguments BuildIndexSearchTerm : simpl never.
 Arguments MatchIndexSearchTerm : simpl never.
@@ -883,10 +883,10 @@ Opaque Initialize_IndexedQueryStructure.
 
 Ltac fields storage :=
   match eval cbv delta [storage] in storage with
-  | let src := ?X in _ => X
+    | let src := ?X in _ => X
   end.
 
-  Ltac prove_extensional_eq :=
+Ltac prove_extensional_eq :=
   clear;
   unfold ExtensionalEq;
   destruct_ifs; first [ solve [intuition] | solve [exfalso; intuition] | idtac ].
@@ -896,26 +896,26 @@ Ltac findMatchingTerm fds s k :=
   match fds with
     | (?fd, ?X) =>
       let H := fresh in assert (H : bindex s = fd) by reflexivity; clear H;
-        k X
+                        k X
     | (?fds1, ?fds2) => findMatchingTerm fds1 s k || findMatchingTerm fds2 s k
   end.
 
 Ltac createTerm f fds tail fs k :=
   match fs with
-  | nil =>
-    k tail
-  | ?s :: ?fs' =>
-    createTerm f fds tail fs' ltac:(fun rest =>
-      findMatchingTerm fds s ltac:(fun X =>
-        k (Some X, rest))
-      || k (@None (f s), rest))
+    | nil =>
+      k tail
+    | ?s :: ?fs' =>
+      createTerm f fds tail fs' ltac:(fun rest =>
+                                        findMatchingTerm fds s ltac:(fun X =>
+                                                                       k (Some X, rest))
+                                                                      || k (@None (f s), rest))
   end.
 
 (* Get the heading of SC, then *)
 Ltac makeTerm fs SC fds tail k :=
   match eval hnf in SC with
-  | Build_Heading ?f =>
-    createTerm f fds tail fs k
+    | Build_Heading ?f =>
+      createTerm f fds tail fs k
   end.
 
 (* Given a storage schema [SC], a filter [F], and a
@@ -941,33 +941,33 @@ Ltac findGoodTerm SC F k :=
 Ltac find_simple_search_term qs_schema idx filter_dec search_term :=
   match type of search_term with
     | BuildIndexSearchTerm ?attr =>
-     let SC := constr:(QSGetNRelSchemaHeading qs_schema idx) in
-              findGoodTerm SC filter_dec
-                           ltac:(fun fds tail =>
-                                   let tail := eval simpl in tail in
-                                       makeTerm attr SC fds tail
-                                                ltac:(fun tm => pose tm; try unify tm search_term;
-                                                      unfold ExtensionalEq, MatchIndexSearchTerm;
-                                                      simpl; intro; try prove_extensional_eq))
+      let SC := constr:(QSGetNRelSchemaHeading qs_schema idx) in
+      findGoodTerm SC filter_dec
+                   ltac:(fun fds tail =>
+                           let tail := eval simpl in tail in
+                               makeTerm attr SC fds tail
+                                        ltac:(fun tm => pose tm; try unify tm search_term;
+                                              unfold ExtensionalEq, MatchIndexSearchTerm;
+                                              simpl; intro; try prove_extensional_eq))
   end.
 
 Ltac implement_QSDeletedTuples find_search_term :=
-match goal with
-    [ H : @DelegateToBag_AbsR ?qs_schema ?indices ?r_o ?r_n
-      |- context[Pick (QSDeletedTuples ?r_o ?idx ?DeletedTuples)] ] =>
-    let filter_dec := eval simpl in (@DecideableEnsembles.dec _ DeletedTuples _) in
-    let idx_search_update_term := eval simpl in (ith_Bounded relName indices idx) in
-    let search_term_type := eval simpl in (BagSearchTermType idx_search_update_term) in
-    let search_term_matcher := eval simpl in (BagMatchSearchTerm idx_search_update_term) in
-        makeEvar search_term_type
-                 ltac: (fun search_term =>
-          let eqv := fresh in
-          assert (ExtensionalEq filter_dec (search_term_matcher search_term)) as eqv;
-            [ find_search_term qs_schema idx filter_dec search_term
-            | let H' := fresh in
-              pose (@refine_BagADT_QSDelete_fst _ _ r_o r_n H idx DeletedTuples _ search_term) as H';
-                setoid_rewrite (H' eqv); clear H' eqv])
-end.
+  match goal with
+      [ H : @DelegateToBag_AbsR ?qs_schema ?indices ?r_o ?r_n
+        |- context[Pick (QSDeletedTuples ?r_o ?idx ?DeletedTuples)] ] =>
+      let filter_dec := eval simpl in (@DecideableEnsembles.dec _ DeletedTuples _) in
+          let idx_search_update_term := eval simpl in (ith_Bounded relName indices idx) in
+              let search_term_type := eval simpl in (BagSearchTermType idx_search_update_term) in
+                  let search_term_matcher := eval simpl in (BagMatchSearchTerm idx_search_update_term) in
+                      makeEvar search_term_type
+                               ltac: (fun search_term =>
+                                        let eqv := fresh in
+                                        assert (ExtensionalEq filter_dec (search_term_matcher search_term)) as eqv;
+                                      [ find_search_term qs_schema idx filter_dec search_term
+                                      | let H' := fresh in
+                                        pose (@refine_BagADT_QSDelete_fst _ _ r_o r_n H idx DeletedTuples _ search_term) as H';
+                                          setoid_rewrite (H' eqv); clear H' eqv])
+  end.
 
 Ltac implement_EnsembleDelete_AbsR find_search_term :=
   match goal with
@@ -977,17 +977,17 @@ Ltac implement_EnsembleDelete_AbsR find_search_term :=
                                                      (EnsembleDelete (GetUnConstrRelation ?r_o ?idx)
                                                                      ?DeletedTuples)) r_n'}]] =>
       let filter_dec := eval simpl in (@DecideableEnsembles.dec _ DeletedTuples _) in
-      let idx_search_update_term := eval simpl in (ith_Bounded relName indices idx) in
-      let search_term_type := eval simpl in (BagSearchTermType idx_search_update_term) in
-      let search_term_matcher := eval simpl in (BagMatchSearchTerm idx_search_update_term) in
-          makeEvar search_term_type
-                   ltac:(fun search_term =>
-                           let eqv := fresh in
-                           assert (ExtensionalEq filter_dec (search_term_matcher search_term)) as eqv;
-                         [ find_search_term qs_schema idx filter_dec search_term
-                         | let H' := fresh in
-                           pose (@refine_BagADT_QSDelete_snd _ _ r_o r_n H idx DeletedTuples _ search_term) as H';
-                             setoid_rewrite (H' eqv); clear H' eqv] )
+          let idx_search_update_term := eval simpl in (ith_Bounded relName indices idx) in
+              let search_term_type := eval simpl in (BagSearchTermType idx_search_update_term) in
+                  let search_term_matcher := eval simpl in (BagMatchSearchTerm idx_search_update_term) in
+                      makeEvar search_term_type
+                               ltac:(fun search_term =>
+                                       let eqv := fresh in
+                                       assert (ExtensionalEq filter_dec (search_term_matcher search_term)) as eqv;
+                                     [ find_search_term qs_schema idx filter_dec search_term
+                                     | let H' := fresh in
+                                       pose (@refine_BagADT_QSDelete_snd _ _ r_o r_n H idx DeletedTuples _ search_term) as H';
+                                         setoid_rewrite (H' eqv); clear H' eqv] )
   end.
 
 Ltac implement_Enumerate_filter find_search_term :=
@@ -995,20 +995,20 @@ Ltac implement_Enumerate_filter find_search_term :=
       [ H : @DelegateToBag_AbsR ?qs_schema ?indices ?r_o ?r_n
         |- context[For (l <- CallBagMethod ?idx {| bindex := "Enumerate"|} ?r_n0 ();
                         (List_Query_In (filter (@DecideableEnsembles.dec _ ?DeletedTuples _) (snd l))
-                                            ?resultComp))]] =>
+                                       ?resultComp))]] =>
       let filter_dec := eval simpl in (@DecideableEnsembles.dec _ DeletedTuples _) in
-      let idx_search_update_term := eval simpl in (ith_Bounded relName indices idx) in
-      let search_term_type := eval simpl in (BagSearchTermType idx_search_update_term) in
-      let search_term_matcher := eval simpl in (BagMatchSearchTerm idx_search_update_term) in
-          makeEvar search_term_type
-                   ltac:(fun search_term =>
-                           let eqv := fresh in
-                           assert (ExtensionalEq filter_dec (search_term_matcher search_term)) as eqv;
-                         [ find_search_term qs_schema idx filter_dec search_term
-                         | let H' := fresh in
-                           pose (@refine_Query_For_In_Find _ _ string _ _ H idx filter_dec
-                                                           search_term resultComp) as H';
-                         setoid_rewrite (H' eqv); clear H'])
+          let idx_search_update_term := eval simpl in (ith_Bounded relName indices idx) in
+              let search_term_type := eval simpl in (BagSearchTermType idx_search_update_term) in
+                  let search_term_matcher := eval simpl in (BagMatchSearchTerm idx_search_update_term) in
+                      makeEvar search_term_type
+                               ltac:(fun search_term =>
+                                       let eqv := fresh in
+                                       assert (ExtensionalEq filter_dec (search_term_matcher search_term)) as eqv;
+                                     [ find_search_term qs_schema idx filter_dec search_term
+                                     | let H' := fresh in
+                                       pose (@refine_Query_For_In_Find _ _ string _ _ H idx filter_dec
+                                                                       search_term resultComp) as H';
+                                         setoid_rewrite (H' eqv); clear H'])
   end.
 
 Ltac implement_Pick_DelegateToBag_AbsR_observer :=
@@ -1018,42 +1018,42 @@ Ltac implement_Pick_DelegateToBag_AbsR_observer :=
       => setoid_rewrite (refine_pick_val (@DelegateToBag_AbsR qs_schema indices r_o) H)
   end.
 
-  Add Parametric Morphism
-      (A : Type)
-      (f : A -> Type)
-      (As : list A)
-      (a : A)
-      (l' : list (ilist f As))
-      : (@Join_Lists A f As a l')
-      with signature
-      (pointwise_relation _ refine) ==> refine
-        as refine_Join_Lists.
-  Proof.
-    unfold pointwise_relation; simpl; intros.
-    induction l'; unfold Join_Lists; simpl.
-    - reflexivity.
-    - rewrite H; setoid_rewrite IHl'; reflexivity.
-  Qed.
+Add Parametric Morphism
+    (A : Type)
+    (f : A -> Type)
+    (As : list A)
+    (a : A)
+    (l' : list (ilist f As))
+: (@Join_Lists A f As a l')
+    with signature
+    (pointwise_relation _ refine) ==> refine
+      as refine_Join_Lists.
+Proof.
+  unfold pointwise_relation; simpl; intros.
+  induction l'; unfold Join_Lists; simpl.
+  - reflexivity.
+  - rewrite H; setoid_rewrite IHl'; reflexivity.
+Qed.
 
 Lemma refine_Join_Enumerate_Swap
       qs_schema BagIndexKeys
-        (ResultT : Type) :
-    forall r_o (r_n : IndexedQueryStructure qs_schema BagIndexKeys),
-      DelegateToBag_AbsR r_o r_n ->
-      forall (idx idx' : BoundedString)
-             (resultComp : _ -> Comp (list ResultT)),
-        refine (l <- CallBagMethod idx {|bindex := "Enumerate" |} r_n ();
-                l' <- (Join_Lists (Build_single_Tuple_list (snd l))
-                                  (fun _ => l <- (CallBagMethod idx' {|bindex := "Enumerate" |} r_n ());
-                                   ret (snd l)));
-                List_Query_In l' resultComp)
-               (l <- CallBagMethod idx' {|bindex := "Enumerate" |} r_n ();
-                l' <- (Join_Lists (Build_single_Tuple_list (snd l))
-                                  (fun _ => l <- (CallBagMethod idx {|bindex := "Enumerate" |} r_n ());
-                                   ret (snd l)));
-                List_Query_In l' (fun tup_pair => (resultComp (icons _ (ilist_hd (ilist_tl tup_pair)) (icons _ (ilist_hd tup_pair) (inil _)))))).
-  Proof.
-  Admitted.
+      (ResultT : Type) :
+  forall r_o (r_n : IndexedQueryStructure qs_schema BagIndexKeys),
+    DelegateToBag_AbsR r_o r_n ->
+    forall (idx idx' : BoundedString)
+           (resultComp : _ -> Comp (list ResultT)),
+      refine (l <- CallBagMethod idx {|bindex := "Enumerate" |} r_n ();
+              l' <- (Join_Lists (Build_single_Tuple_list (snd l))
+                                (fun _ => l <- (CallBagMethod idx' {|bindex := "Enumerate" |} r_n ());
+                                 ret (snd l)));
+              List_Query_In l' resultComp)
+             (l <- CallBagMethod idx' {|bindex := "Enumerate" |} r_n ();
+              l' <- (Join_Lists (Build_single_Tuple_list (snd l))
+                                (fun _ => l <- (CallBagMethod idx {|bindex := "Enumerate" |} r_n ());
+                                 ret (snd l)));
+              List_Query_In l' (fun tup_pair => (resultComp (icons _ (ilist_hd (ilist_tl tup_pair)) (icons _ (ilist_hd tup_pair) (inil _)))))).
+Proof.
+Admitted.
 
 (* implement_In' implements [UnConstrQuery_In] in a variety of contexts. *)
 Ltac implement_In' :=
@@ -1088,161 +1088,157 @@ Ltac implement_In :=
   repeat implement_In'.
 
 
-  Fixpoint Join_ListsT (Ts : list Type) : Type
-    :=
-      match Ts with
-        | [] => unit
-        | [A] => A
-        | A :: Cs => prod A (Join_ListsT Cs)
-      end.
-
-  Lemma ExtensionalEq_andb {A} :
-    forall (f g f' g' : A -> bool),
-      ExtensionalEq f f'
-      -> ExtensionalEq g g'
-      -> ExtensionalEq (fun a => f a && g a) (fun a => f' a && g' a).
-  Proof.
-    unfold ExtensionalEq; intros; congruence.
-  Qed.
-
-  Lemma ExtensionalEq_andb_true {A} :
-    forall (f f' : A -> bool),
-      ExtensionalEq f f'
-      -> ExtensionalEq f (fun a => f' a && (fun _ => true) a).
-  Proof.
-    unfold ExtensionalEq; intros.
-    rewrite andb_true_r; apply H.
-  Qed.
-
-  Ltac split_filters k :=
-    match goal with
-      | |- ExtensionalEq (fun a => (@?f a) && (@?g a)) ?b =>
-        let fT := type of f in
-        let gT := type of g in
-        makeEvar
-          fT
-          ltac:(fun f' =>
-                  makeEvar gT ltac:(fun g' =>
-                                      apply (@ExtensionalEq_andb _ f g f' g');
-                                    [ first [split_filters | k ] | first [split_filters | k]] ))
-      | |- ExtensionalEq (fun a => (@?f a)) ?b =>
-        let fT := type of f in
-        makeEvar
-          fT
-          ltac:(fun f' => k)
+Fixpoint Join_ListsT (Ts : list Type) : Type
+  :=
+    match Ts with
+      | [] => unit
+      | [A] => A
+      | A :: Cs => prod A (Join_ListsT Cs)
     end.
 
-  (* Convert List_Query_In Where Clauses into a filter using search terms. *)
-  Ltac convert_Where_to_search_term :=
-    (* First replace Where clauses with test functions. *)
-    simpl; repeat (setoid_rewrite refine_List_Query_In_Where;
-                   instantiate (1 := _)); simpl;
-    (* Combine different filters into a single function. *)
-    repeat setoid_rewrite <- filter_and;
-    (* Now break the functions up again and find search term replacements for each. *)
-    match goal with
-        |- context [List_Query_In (filter ?f _) _] =>
-        let T := type of f in
-        makeEvar T
-                 ltac:(fun g =>
-                         let eqv := fresh in
-                         assert (ExtensionalEq f g) as eqv;
-                       [ apply ExtensionalEq_andb_true; split_filters idtac
-                       | setoid_rewrite (filter_by_equiv f g eqv)])
-    end.
+Lemma ExtensionalEq_andb {A} :
+  forall (f g f' g' : A -> bool),
+    ExtensionalEq f f'
+    -> ExtensionalEq g g'
+    -> ExtensionalEq (fun a => f a && g a) (fun a => f' a && g' a).
+Proof.
+  unfold ExtensionalEq; intros; congruence.
+Qed.
 
-  Ltac equate X Y := let H := fresh in assert (H : X = Y) by reflexivity; clear H.
+Lemma ExtensionalEq_andb_true {A} :
+  forall (f f' : A -> bool),
+    ExtensionalEq f f'
+    -> ExtensionalEq f (fun a => f' a && (fun _ => true) a).
+Proof.
+  unfold ExtensionalEq; intros.
+  rewrite andb_true_r; apply H.
+Qed.
 
-    Definition unit_Heading :=
-      {| Attributes := unit;
-         Domain := fun _ => unit |}.
+Ltac split_filters k :=
+  match goal with
+    | |- ExtensionalEq (fun a => (@?f a) && (@?g a)) ?b =>
+      let fT := type of f in
+      let gT := type of g in
+      makeEvar
+        fT
+        ltac:(fun f' =>
+                makeEvar gT ltac:(fun g' =>
+                                    apply (@ExtensionalEq_andb _ f g f' g');
+                                  [ first [split_filters | k ] | first [split_filters | k]] ))
+    | |- ExtensionalEq (fun a => (@?f a)) ?b => k
+  end.
 
-    Definition unit_Tuple : @Tuple unit_Heading := id.
+(* Convert List_Query_In Where Clauses into a filter using search terms. *)
+Ltac convert_Where_to_search_term :=
+  (* First replace Where clauses with test functions. *)
+  simpl; repeat (setoid_rewrite refine_List_Query_In_Where;
+                 instantiate (1 := _)); simpl;
+  (* Combine different filters into a single function. *)
+  repeat setoid_rewrite <- filter_and;
+  (* Now break the functions up again and find search term replacements for each. *)
+  match goal with
+      |- context [List_Query_In (filter ?f _) _] =>
+      let T := type of f in
+      makeEvar T
+               ltac:(fun g =>
+                       let eqv := fresh in
+                       assert (ExtensionalEq f g) as eqv;
+                     [ apply ExtensionalEq_andb_true; split_filters idtac
+                     | setoid_rewrite (filter_by_equiv f g eqv)])
+  end.
 
-    Ltac get_ithDefault f n k :=
-      match type of f with
-        | ilist (@Tuple) ?A -> ?C =>
-          let G := fresh "G" in
-          let p := fresh "p" in
-          let H := fresh "H" in
-          let proj := fresh "proj" in
-          let proj := eval simpl in
-          (fun b : ilist (@Tuple) A => ith_default unit_Heading unit_Tuple b n) in
+Ltac equate X Y := let H := fresh in assert (H : X = Y) by reflexivity; clear H.
+
+Definition unit_Heading :=
+  {| Attributes := unit;
+     Domain := fun _ => unit |}.
+
+Definition unit_Tuple : @Tuple unit_Heading := id.
+
+Ltac get_ithDefault f n k :=
+  match type of f with
+    | ilist (@Tuple) ?A -> ?C =>
+      let G := fresh "G" in
+      let p := fresh "p" in
+      let H := fresh "H" in
+      let proj := fresh "proj" in
+      let proj := eval simpl in
+      (fun b : ilist (@Tuple) A => ith_default unit_Heading unit_Tuple b n) in
           evar (G : @Tuple (nth_default unit_Heading A n) -> C);
-             assert (H : forall p,
-                          f p = G (proj p)) by
-              (subst G; intro p;
-               let p' := eval simpl in (proj p) in
-                   pattern p';
-               match goal with
-                 | [ |- (fun t => @?f t = @?g t) _ ] => equate g f; reflexivity
-               end); clear H;
+        assert (H : forall p,
+                      f p = G (proj p)) by
+          (subst G; intro p;
+           let p' := eval simpl in (proj p) in
+               pattern p';
+           match goal with
+             | [ |- (fun t => @?f t = @?g t) _ ] => equate g f; reflexivity
+           end); clear H;
         let G' := eval unfold G in G in clear G; k G'
-      end.
+  end.
 
-    Ltac get_ithDefault_pair f m n k :=
-      match type of f with
-        | ilist (@Tuple) ?A -> ?C =>
-          let G := fresh "G" in
-          let p := fresh "p" in
-          let H := fresh "H" in
-          let proj1 := fresh "proj" in
-          let proj2 := fresh "proj" in
-          let proj1 := eval simpl in
-          (fun b : ilist (@Tuple) A => ith_default unit_Heading unit_Tuple b m) in
+Ltac get_ithDefault_pair f m n k :=
+  match type of f with
+    | ilist (@Tuple) ?A -> ?C =>
+      let G := fresh "G" in
+      let p := fresh "p" in
+      let H := fresh "H" in
+      let proj1 := fresh "proj" in
+      let proj2 := fresh "proj" in
+      let proj1 := eval simpl in
+      (fun b : ilist (@Tuple) A => ith_default unit_Heading unit_Tuple b m) in
           let proj2 := eval simpl in
           (fun b : ilist (@Tuple) A => ith_default unit_Heading unit_Tuple b n)
             in evar (G : @Tuple (nth_default unit_Heading A m)
                          -> @Tuple (nth_default unit_Heading A n)
                          -> C);
-             assert (H : forall p,
-                           f p = G (proj1 p) (proj2 p)) by
+            assert (H : forall p,
+                          f p = G (proj1 p) (proj2 p)) by
               ( subst G; intro p;
-               let p1 := eval simpl in (proj1 p) in
-               let p2 := eval simpl in (proj2 p) in
-               pattern p1, p2;
-                 match goal with
-                   | [ |- (fun t t' => @?f t t' = @?g t t') _ _ ] => equate f g; reflexivity
-                 end); clear H;
-             let G' := eval unfold G in G in clear G; k G'
-      end.
-
- (* Build pairs of fields + their values. *)
-    Ltac findGoodTerm_dep SC F k :=
-  match F with
-  | fun (a : ?T) b => ?[@?f a b] =>
-    match type of f with
-    | forall a b, {@?X a = _!?fd} + {_} => k (fd, X) (fun _ : @Tuple SC => true)
-    | forall a b, {_!?fd = @?X a} + {_} => k (fd, X) (fun _ : @Tuple SC => true)
-    | forall a b, {@?X a = _``?fd} + {_} => k (fd, X) (fun _ : @Tuple SC => true)
-    | forall a b, {_``?fd = @?X a} + {_} => k (fd, X) (fun _ : @Tuple SC => true)
-    end
-  | fun (a : ?T) b => (@?f a b) && (@?g a b) =>
-    findGoodTerm_dep SC f ltac:(fun fds1 tail1 =>
-      findGoodTerm_dep SC g ltac:(fun fds2 tail2 =>
-        k (fds1, fds2) (fun tup : @Tuple SC => (tail1 tup) && (tail2 tup))))
-  | _ => k tt F
+                let p1 := eval simpl in (proj1 p) in
+                    let p2 := eval simpl in (proj2 p) in
+                        pattern p1, p2;
+                match goal with
+                  | [ |- (fun t t' => @?f t t' = @?g t t') _ _ ] => equate f g; reflexivity
+                end); clear H;
+            let G' := eval unfold G in G in clear G; k G'
   end.
 
-    (* Build search a search term from the list of attribute + value pairs in fs. *)
+(* Build pairs of fields + their values. *)
+Ltac findGoodTerm_dep SC F k :=
+  match F with
+    | fun (a : ?T) b => ?[@?f a b] =>
+      match type of f with
+        | forall a b, {@?X a = _!?fd} + {_} => k (fd, X) (fun _ : @Tuple SC => true)
+        | forall a b, {_!?fd = @?X a} + {_} => k (fd, X) (fun _ : @Tuple SC => true)
+        | forall a b, {@?X a = _``?fd} + {_} => k (fd, X) (fun _ : @Tuple SC => true)
+        | forall a b, {_``?fd = @?X a} + {_} => k (fd, X) (fun _ : @Tuple SC => true)
+      end
+    | fun (a : ?T) b => (@?f a b) && (@?g a b) =>
+      findGoodTerm_dep SC f ltac:(fun fds1 tail1 =>
+                                    findGoodTerm_dep SC g ltac:(fun fds2 tail2 =>
+                                                                  k (fds1, fds2) (fun tup : @Tuple SC => (tail1 tup) && (tail2 tup))))
+    | _ => k tt F
+  end.
+
+(* Build search a search term from the list of attribute + value pairs in fs. *)
 Ltac createTerm_dep dom fs f fds tail k :=
   match fs with
-  | nil =>
-    k (fun x : dom => tail)
-  | ?s :: ?fs' =>
-    createTerm_dep dom fs' f fds tail
-      ltac:(fun rest =>
-               findMatchingTerm fds s
-                   ltac:(fun X =>
-                           k (fun x : dom => (Some (X x), rest x)))
-                          || k (fun x : dom => (@None (f s), rest x)))
+    | nil =>
+      k (fun x : dom => tail)
+    | ?s :: ?fs' =>
+      createTerm_dep dom fs' f fds tail
+                     ltac:(fun rest =>
+                             findMatchingTerm fds s
+                                              ltac:(fun X =>
+                                                      k (fun x : dom => (Some (X x), rest x)))
+                                                     || k (fun x : dom => (@None (f s), rest x)))
   end.
 
 (* Get the heading of [SC] before building the search term. *)
 Ltac makeTerm_dep dom fs SC fds tail k :=
   match eval hnf in SC with
-  | Build_Heading ?f =>
-    createTerm_dep dom fs f fds tail k
+    | Build_Heading ?f =>
+      createTerm_dep dom fs f fds tail k
   end.
 
 Definition Dep_SearchTerm_Wrapper {A} {heading}
@@ -1279,164 +1275,332 @@ Ltac find_equivalent_tuple schemas heading k :=
   end.
 
 Ltac find_equivalent_search_term_pair m n build_search_term_dep :=
-match goal with
-    [ H : @DelegateToBag_AbsR ?qs_schema ?indices ?r_o ?r_n
-      |- ExtensionalEq ?f _ ] =>
-    get_ithDefault_pair f m n
-      ltac:(fun filter_dec =>
-        let dom := match type of filter_dec with
-                     | ?A -> ?B -> bool => constr:(A)
-                   end in
-        let heading := match type of filter_dec with
-                         | ?A -> @Tuple ?heading -> bool => constr:(heading)
-                       end in
-        let schemas := eval simpl in (qschemaSchemas qs_schema) in
-            find_equivalent_tuple schemas heading
-              ltac:(fun id => let idx' := constr:({| bindex := id |} : BoundedIndex (map relName (qschemaSchemas qs_schema)))
-                              in let idx := eval simpl in idx' in
-    let idx_search_update_term := eval simpl in (ith_Bounded relName indices idx) in
-    let search_term_type := eval simpl in (BagSearchTermType idx_search_update_term) in
-        let search_term_matcher := eval simpl in (BagMatchSearchTerm idx_search_update_term) in
-        makeEvar (dom -> search_term_type)
-                 ltac: (fun search_term =>
-                          let eqv := fresh in
-                          assert (forall a b, filter_dec a b
-                                                = search_term_matcher (search_term a) b) as eqv;
-                        [ build_search_term_dep qs_schema idx
-                          dom filter_dec search_term
-                        | match goal with
-                            |- ExtensionalEq ?f ?search_term' =>
-                            match type of f with
-                                | ?A -> _ =>
-                                  unify search_term' (fun a : A => search_term_matcher (search_term (ith_default unit_Heading unit_Tuple a m))
-            ((ith_default unit_Heading unit_Tuple a n)))
-                            end
-                                                  end;
-                          unfold ExtensionalEq in *; intros;
-                          simpl in *; rewrite eqv; reflexivity
-]))) end.
+  match goal with
+      [ H : @DelegateToBag_AbsR ?qs_schema ?indices ?r_o ?r_n
+        |- ExtensionalEq ?f _ ] =>
+      get_ithDefault_pair f m n
+                          ltac:(fun filter_dec =>
+                                  let dom := match type of filter_dec with
+                                               | ?A -> ?B -> bool => constr:(A)
+                                             end in
+                                  let heading := match type of filter_dec with
+                                                   | ?A -> @Tuple ?heading -> bool => constr:(heading)
+                                                 end in
+                                  let schemas := eval simpl in (qschemaSchemas qs_schema) in
+                                      find_equivalent_tuple schemas heading
+                                                            ltac:(fun id => let idx' := constr:({| bindex := id |} : BoundedIndex (map relName (qschemaSchemas qs_schema)))
+                                                                            in let idx := eval simpl in idx' in
+                                                                                   let idx_search_update_term := eval simpl in (ith_Bounded relName indices idx) in
+                                                                                       let search_term_type := eval simpl in (BagSearchTermType idx_search_update_term) in
+                                                                                           let search_term_matcher := eval simpl in (BagMatchSearchTerm idx_search_update_term) in
+                                                                                               makeEvar (dom -> search_term_type)
+                                                                                                        ltac: (fun search_term =>
+                                                                                                                 let eqv := fresh in
+                                                                                                                 assert (forall a b, filter_dec a b
+                                                                                                                                     = search_term_matcher (search_term a) b) as eqv;
+                                                                                                               [ build_search_term_dep qs_schema idx
+                                                                                                                                       dom filter_dec search_term
+                                                                                                               | match goal with
+                                                                                                                     |- ExtensionalEq ?f ?search_term' =>
+                                                                                                                     match type of f with
+                                                                                                                       | ?A -> _ =>
+                                                                                                                         unify search_term' (fun a : A => search_term_matcher (search_term (ith_default unit_Heading unit_Tuple a m))
+                                                                                                                                                                              ((ith_default unit_Heading unit_Tuple a n)))
+                                                                                                                     end
+                                                                                                                 end;
+                                                                                                                 unfold ExtensionalEq in *; intros;
+                                                                                                                 simpl in *; rewrite eqv; reflexivity
+                                                                                                               ]))) end.
 
 Ltac find_equivalent_search_term m build_search_term :=
-match goal with
-    [ H : @DelegateToBag_AbsR ?qs_schema ?indices ?r_o ?r_n
-      |- ExtensionalEq ?f _ ] =>
-    get_ithDefault f m
-      ltac:(fun filter_dec =>
-        let heading := match type of filter_dec with
-                         | @Tuple ?heading -> bool => constr:(heading)
-                       end in
-        let schemas := eval simpl in (qschemaSchemas qs_schema) in
-            find_equivalent_tuple schemas heading
-              ltac:(fun id => let idx' := constr:({| bindex := id |} : BoundedIndex (map relName (qschemaSchemas qs_schema)))
-                              in let idx := eval simpl in idx' in
-    let idx_search_update_term := eval simpl in (ith_Bounded relName indices idx) in
-    let search_term_type := eval simpl in (BagSearchTermType idx_search_update_term) in
-        let search_term_matcher := eval simpl in (BagMatchSearchTerm idx_search_update_term) in
-        makeEvar (search_term_type)
-                 ltac: (fun search_term =>
-                          let eqv := fresh in
-                          assert (forall a, filter_dec a
-                                                = search_term_matcher search_term a) as eqv;
-                        [ build_search_term qs_schema idx
-                          filter_dec search_term
-                        | match goal with
-                              |- ExtensionalEq ?f ?search_term' =>
-                              match type of f with
-                                | ?A -> _ =>
-                                  unify search_term' (fun a : A => search_term_matcher search_term (ith_default unit_Heading unit_Tuple a m))
-                              end
-                          end;
-                          unfold ExtensionalEq in *; intros;
-                          simpl in *; rewrite eqv; reflexivity
-]))) end.
+  match goal with
+      [ H : @DelegateToBag_AbsR ?qs_schema ?indices ?r_o ?r_n
+        |- ExtensionalEq ?f _ ] =>
+      get_ithDefault f m
+                     ltac:(fun filter_dec =>
+                             let heading := match type of filter_dec with
+                                              | @Tuple ?heading -> bool => constr:(heading)
+                                            end in
+                             let schemas := eval simpl in (qschemaSchemas qs_schema) in
+                                 find_equivalent_tuple schemas heading
+                                                       ltac:(fun id => let idx' := constr:({| bindex := id |} : BoundedIndex (map relName (qschemaSchemas qs_schema)))
+                                                                       in let idx := eval simpl in idx' in
+                                                                              let idx_search_update_term := eval simpl in (ith_Bounded relName indices idx) in
+                                                                                  let search_term_type := eval simpl in (BagSearchTermType idx_search_update_term) in
+                                                                                      let search_term_matcher := eval simpl in (BagMatchSearchTerm idx_search_update_term) in
+                                                                                          makeEvar (search_term_type)
+                                                                                                   ltac: (fun search_term =>
+                                                                                                            let eqv := fresh in
+                                                                                                            assert (forall a, filter_dec a
+                                                                                                                              = search_term_matcher search_term a) as eqv;
+                                                                                                          [ build_search_term qs_schema idx
+                                                                                                                              filter_dec search_term
+                                                                                                          | match goal with
+                                                                                                                |- ExtensionalEq ?f ?search_term' =>
+                                                                                                                match type of f with
+                                                                                                                  | ?A -> _ =>
+                                                                                                                    unify search_term' (fun a : A => search_term_matcher search_term (ith_default unit_Heading unit_Tuple a m))
+                                                                                                                end
+                                                                                                            end;
+                                                                                                            unfold ExtensionalEq in *; intros;
+                                                                                                            simpl in *; rewrite eqv; reflexivity
+                                                                                                          ]))) end.
 
 
 Corollary refine_Join_Lists_filter_filter_search_term_snd_dep'
           qs_schema BagIndexKeys
-        (ResultT : Type) :
-    forall (r_n : IndexedQueryStructure qs_schema BagIndexKeys)
-           idx idx'
-           (search_pattern : _ -> _)
-           (resultComp : ilist (@Tuple) [_; _] -> Comp (list ResultT))
-           filter_rest st,
-      refine (cl <- CallBagMethod idx {| bindex := "Find" |} r_n st;
-              l' <- (Join_Lists (Build_single_Tuple_list (snd cl))
-                                (fun _ => l <- CallBagMethod idx' {| bindex := "Enumerate" |} r_n ();
-                                 ret (snd l)));
-              List_Query_In (filter (fun a : ilist (@Tuple) [_ ; _] => BagMatchSearchTerm _ (search_pattern (ilist_tl a)) (ilist_hd a) && filter_rest a) l')
-                            resultComp)
-             (cl <- CallBagMethod idx {| bindex := "Find" |} r_n st;
-              l' <- (Join_Lists (Build_single_Tuple_list (snd cl))
-                                (fun tup => l <- CallBagMethod idx' {| bindex := "Find" |} r_n (search_pattern tup);
-                                             ret (snd l)));
-                      List_Query_In (filter filter_rest l') resultComp).
-  Proof.
-    intros; f_equiv; intro;
-    apply refine_Join_Lists_filter_search_term_snd_dep.
-  Qed.
+          (ResultT : Type) :
+  forall (r_n : IndexedQueryStructure qs_schema BagIndexKeys)
+         idx idx'
+         (search_pattern : _ -> _)
+         (resultComp : ilist (@Tuple) [_; _] -> Comp (list ResultT))
+         filter_rest st,
+    refine (cl <- CallBagMethod idx {| bindex := "Find" |} r_n st;
+            l' <- (Join_Lists (Build_single_Tuple_list (snd cl))
+                              (fun _ => l <- CallBagMethod idx' {| bindex := "Enumerate" |} r_n ();
+                               ret (snd l)));
+            List_Query_In (filter (fun a : ilist (@Tuple) [_ ; _] => BagMatchSearchTerm _ (search_pattern (ilist_tl a)) (ilist_hd a) && filter_rest a) l')
+                          resultComp)
+           (cl <- CallBagMethod idx {| bindex := "Find" |} r_n st;
+            l' <- (Join_Lists (Build_single_Tuple_list (snd cl))
+                              (fun tup => l <- CallBagMethod idx' {| bindex := "Find" |} r_n (search_pattern tup);
+                               ret (snd l)));
+            List_Query_In (filter filter_rest l') resultComp).
+Proof.
+  intros; f_equiv; intro;
+  apply refine_Join_Lists_filter_search_term_snd_dep.
+Qed.
 
-  Ltac convert_filter_to_find':=
-    try match goal with
-            |- context[filter (fun a => (_ && _) && true) _] =>
-            setoid_rewrite <- andb_assoc; simpl
-        end;
+Ltac convert_filter_to_find':=
+  try match goal with
+          |- context[filter (fun a => (_ && _) && true) _] =>
+          setoid_rewrite <- andb_assoc; simpl
+      end;
+  match goal with
+    | H : @DelegateToBag_AbsR ?qs_schema ?indices ?r_o ?r_n
+      |- context[l <- CallBagMethod ?idx ``("Enumerate") ?r_n ();
+                  List_Query_In (filter (fun a => MatchIndexSearchTerm ?st (ilist_hd a) && @?filter_rest a)
+                                        (Build_single_Tuple_list (snd l))) ?resultComp] =>
+      let b := fresh in
+      pose proof (@refine_Query_For_In_Find_single _ _ _ r_o r_n H idx st resultComp filter_rest) as b;
+        simpl in b; setoid_rewrite b; clear b
+
+    | H : @DelegateToBag_AbsR ?qs_schema ?indices ?r_o ?r_n
+      |- context[l <- CallBagMethod ?idx ``("Enumerate") ?r_n ();
+                  l' <- Join_Lists (Build_single_Tuple_list (snd l)) ?cl;
+                  List_Query_In (filter (fun a => MatchIndexSearchTerm ?st (ilist_hd (ilist_tl a)) && @?filter_rest a)
+                                        l') ?resultComp] =>
+      let b := fresh in
+      pose proof (fun foo => @refine_Join_Lists_filter_search_term_fst _ _ _ r_n idx _ cl st resultComp foo filter_rest) as b;
+        simpl in b; setoid_rewrite b;
+        [ clear b
+        | match goal with
+            | |- context [CallBagMethod ?idx' ``("Enumerate") _ _] =>
+              intros; eapply (realizeable_Enumerate (r_o := r_o) (r_n := r_n) idx' H)
+            | |- context [CallBagMethod ?idx' ``("Find") _ _] =>
+              intros; eapply (realizeable_Find (r_o := r_o) (r_n := r_n) idx' H)
+          end]
+    | H : @DelegateToBag_AbsR ?qs_schema ?indices ?r_o ?r_n
+      |- context[l <- CallBagMethod ?idx ``("Find") ?r_n ?st;
+                  l' <- Join_Lists (Build_single_Tuple_list (snd l))
+                     (fun _ : ilist (@Tuple) [?heading] =>
+                        l <- CallBagMethod ?idx' ``("Enumerate") ?r_n ();
+                      ret (snd l));
+                  List_Query_In (filter (fun a => MatchIndexSearchTerm (Dep_SearchTerm_Wrapper ?st' (ilist_hd (ilist_tl a)))
+                                                                       (ilist_hd a) && @?filter_rest a) l') ?resultComp] =>
+      let b := fresh in
+      pose proof (@refine_Join_Lists_filter_filter_search_term_snd_dep' _ _ _ r_n idx idx'
+                                                                        (fun a => Dep_SearchTerm_Wrapper st' (ilist_hd a))
+                                                                        resultComp filter_rest st) as b;
+        unfold Dep_SearchTerm_Wrapper in b; simpl in b; setoid_rewrite b; clear b
+    (* The final case replaces the last filter and the Return statement. *)
+    | _ => setoid_rewrite filter_true; setoid_rewrite refine_List_Query_In_Return
+  end.
+
+Ltac convert_filter_to_find :=
+  simpl; repeat convert_filter_to_find'.
+
+(* This also implements Fors *)
+Ltac Implement_Aggregates :=
+  repeat
     match goal with
-      | H : @DelegateToBag_AbsR ?qs_schema ?indices ?r_o ?r_n
-        |- context[l <- CallBagMethod ?idx ``("Enumerate") ?r_n ();
-                    List_Query_In (filter (fun a => MatchIndexSearchTerm ?st (ilist_hd a) && @?filter_rest a)
-                                          (Build_single_Tuple_list (snd l))) ?resultComp] =>
-        let b := fresh in
-        pose proof (@refine_Query_For_In_Find_single _ _ _ r_o r_n H idx st resultComp filter_rest) as b;
-          simpl in b; setoid_rewrite b; clear b
-
-      | H : @DelegateToBag_AbsR ?qs_schema ?indices ?r_o ?r_n
-        |- context[l <- CallBagMethod ?idx ``("Enumerate") ?r_n ();
-                    l' <- Join_Lists (Build_single_Tuple_list (snd l)) ?cl;
-                    List_Query_In (filter (fun a => MatchIndexSearchTerm ?st (ilist_hd (ilist_tl a)) && @?filter_rest a)
-                                          l') ?resultComp] =>
-        let b := fresh in
-        pose proof (fun foo => @refine_Join_Lists_filter_search_term_fst _ _ _ r_n idx _ cl st resultComp foo filter_rest) as b;
-          simpl in b; setoid_rewrite b;
-          [ clear b
-          | match goal with
-              | |- context [CallBagMethod ?idx' ``("Enumerate") _ _] =>
-                intros; eapply (realizeable_Enumerate (r_o := r_o) (r_n := r_n) idx' H)
-              | |- context [CallBagMethod ?idx' ``("Find") _ _] =>
-                intros; eapply (realizeable_Find (r_o := r_o) (r_n := r_n) idx' H)
-            end]
-      | H : @DelegateToBag_AbsR ?qs_schema ?indices ?r_o ?r_n
-        |- context[l <- CallBagMethod ?idx ``("Find") ?r_n ?st;
-                    l' <- Join_Lists (Build_single_Tuple_list (snd l))
-                       (fun _ : ilist (@Tuple) [?heading] =>
-                          l <- CallBagMethod ?idx' ``("Enumerate") ?r_n ();
-                        ret (snd l));
-                    List_Query_In (filter (fun a => MatchIndexSearchTerm (Dep_SearchTerm_Wrapper ?st' (ilist_hd (ilist_tl a)))
-                                                                         (ilist_hd a) && @?filter_rest a) l') ?resultComp] =>
-        let b := fresh in
-        pose proof (@refine_Join_Lists_filter_filter_search_term_snd_dep' _ _ _ r_n idx idx'
-                                                                          (fun a => Dep_SearchTerm_Wrapper st' (ilist_hd a))
-                                                                          resultComp filter_rest st) as b;
-          unfold Dep_SearchTerm_Wrapper in b; simpl in b; setoid_rewrite b; clear b
-      (* The final case replaces the last filter and the Return statement. *)
-      | _ => setoid_rewrite filter_true; setoid_rewrite refine_List_Query_In_Return
+      | |- context[For _] => setoid_rewrite refine_For_List
+      | |- context[Count _] => setoid_rewrite refine_Count
     end.
 
-  Ltac convert_filter_to_find :=
-    simpl; repeat convert_filter_to_find'.
+(* Commits the database at the end of a method call. *)
+Ltac commit :=
+  match goal with
+    | [H : @DelegateToBag_AbsR ?qs_schema ?indices ?r_o ?r_n
+       |- context[{r_n' : IndexedQueryStructure ?qs_schema ?indices | DelegateToBag_AbsR ?r_o r_n'}] ]
+      => setoid_rewrite (refine_pick_val (@DelegateToBag_AbsR qs_schema indices r_o) H);
+        simplify with monad laws
+  end.
 
-  (* This also implements Fors *)
-  Ltac Implement_Aggregates :=
-    repeat
-      match goal with
-        | |- context[For _] => setoid_rewrite refine_For_List
-        | |- context[Count _] => setoid_rewrite refine_Count
-      end.
+Global Opaque CallBagMethod.
+Global Opaque CallBagConstructor.
 
-  (* Commits the database at the end of a method call. *)
-  Ltac commit :=
+Arguments icons {A} {B} {a} {As} _ _.
+Arguments CallBagConstructor {heading} name {index} cidx _.
+
+
+Fixpoint Initialize_IndexedQueryStructureImpls'
+         {indices}
+         Index DelegateImpls
+         {struct Index}
+: @Build_IndexedQueryStructure_Impl_cRep indices Index DelegateImpls :=
+  match Index return
+        forall DelegateImpls, Build_IndexedQueryStructure_Impl_cRep Index DelegateImpls
+  with
+    | inil => i2nil _
+    | icons a b As Bs => fun DelegateImpls =>
+                           i2cons _
+                                  (ComputationalADT.cConstructors (ilist_hd DelegateImpls)
+                                                                  {| bindex := "Empty" |} ())
+                                  (Initialize_IndexedQueryStructureImpls' Bs (ilist_tl DelegateImpls))
+  end DelegateImpls.
+
+Ltac higher_order_1_reflexivity'' :=
+  let x := match goal with |- ?R (ret ?x) (ret (?f ?a)) => constr:(x) end in
+  let f := match goal with |- ?R (ret ?x) (ret (?f ?a)) => constr:(f) end in
+  let a := match goal with |- ?R (ret ?x) (ret (?f ?a)) => constr:(a) end in
+  let x' := (eval pattern a in x) in
+  let f' := match x' with ?f' _ => constr:(f') end in
+  unify f f';
+    cbv beta;
+    solve [apply reflexivity].
+
+Ltac higher_order_2_reflexivity'' :=
+  let x := match goal with |- ?R (ret ?x) (ret (?f ?a ?b)) => constr:(x) end in
+  let f := match goal with |- ?R (ret ?x) (ret (?f ?a ?b)) => constr:(f) end in
+  let a := match goal with |- ?R (ret ?x) (ret (?f ?a ?b)) => constr:(a) end in
+  let b := match goal with |- ?R (ret ?x) (ret (?f ?a ?b)) => constr:(b) end in
+  let x' := (eval pattern a, b in x) in
+  let f' := match x' with ?f' _ _ => constr:(f') end in
+  unify f f';
+    cbv beta;
+    solve [apply reflexivity].
+
+Ltac implement_bag_constructors :=
+  repeat match goal with
+           | |- context[ Pick (fun r_n : Build_IndexedQueryStructure_Impl_cRep ?Index ?DelegateImpls =>
+                                 Build_IndexedQueryStructure_Impl_AbsR' ?ValidImpl ?r_o r_n)] =>
+             refine pick val (Initialize_IndexedQueryStructureImpls' Index DelegateImpls);
+               [ higher_order_2_reflexivity'' |
+                 unfold Build_IndexedQueryStructure_Impl_AbsR', Build_IndexedQueryStructure_Impl_AbsR'';
+                   eapply Iterate_Dep_Type_BoundedIndex_equiv_1; simpl; intuition ]
+
+           | |- context[CallBagConstructor ?ridx ?cidx ?d] =>
+             match goal with
+                 |- appcontext[Build_IndexedQueryStructure_Impl_AbsR'
+                                 (qs_schema := ?qs_schema)
+                                 (Index := ?Index)
+                                 (DelegateImpls := ?DelegateImpls) ?ValidImpl] =>
+                 let r_o' := fresh "r_o'" in
+                 let AbsR_r_o' := fresh "AbsR_r_o'" in
+                 let refines_r_o' := fresh "refines_r_o'" in
+                 destruct (@refine_BagImplConstructor
+                             qs_schema Index DelegateImpls
+                             (fun idx =>
+                                ValidImpl (map_IndexedQS_idx' Index idx))
+                             {|bindex := ridx |} cidx d) as
+                     [r_o' [refines_r_o' AbsR_r_o']];
+                   unfold map_IndexedQS_idx' in refines_r_o', AbsR_r_o'; simpl in refines_r_o', AbsR_r_o';
+                   setoid_rewrite refines_r_o'; simpl in *; simplify with monad laws; simpl
+             end
+         end.
+
+Definition Join_Lists'
+           {A : Type} {f : A -> Type} {As : list A} {a : A}
+           (l : list (ilist f As)) (c : ilist f As -> list (f a))
+  := flatten (map
+                (fun l' => map (fun fa : f a => icons fa l') (c l')) l).
+
+Lemma Join_Lists_Impl {A : Type} {f : A -> Type} {As : list A} {a : A}
+: forall (l : list (ilist f As))
+         (c : ilist f As -> Comp (list (f a)))
+         (c' : ilist f As -> list (f a)),
+    (forall a', refine (c a') (ret (c' a')))
+    -> refine (Join_Lists l c) (ret (Join_Lists' l c')).
+Proof.
+  induction l; unfold Join_Lists, Join_Lists'; simpl; intros.
+  - reflexivity.
+  - rewrite H; simplify with monad laws.
+    setoid_rewrite IHl; eauto; simplify with monad laws.
+    reflexivity.
+Qed.
+
+Ltac implement_bag_methods :=
+  unfold Build_IndexedQueryStructure_Impl_AbsR' in *;
+  repeat
     match goal with
-      | [H : @DelegateToBag_AbsR ?qs_schema ?indices ?r_o ?r_n
-         |- context[{r_n' : IndexedQueryStructure ?qs_schema ?indices | DelegateToBag_AbsR ?r_o r_n'}] ]
-        => setoid_rewrite (refine_pick_val (@DelegateToBag_AbsR qs_schema indices r_o) H);
-          simplify with monad laws
+      | |- refine (ret _) (ret (?f ?a ?b)) => higher_order_2_reflexivity''
+      | |- refine (ret _) (ret (?f ?a)) => higher_order_1_reflexivity''
+
+      |  [ H : Build_IndexedQueryStructure_Impl_AbsR'' (qs_schema := ?qs_schema)
+                                                       (DelegateImpls := ?DelegateImpl)
+                                                       (fun idx => ?ValidImpl (map_IndexedQS_idx' ?Index idx)) ?r_o ?r_n
+           |- context[
+                  { r_n' | Build_IndexedQueryStructure_Impl_AbsR'' (fun idx => ?ValidImpl (map_IndexedQS_idx' ?Index idx)) ?r_o r_n'}
+                ]] => refine pick val _;
+           [ simplify with monad laws |
+             eapply H]
+
+      | H : Build_IndexedQueryStructure_Impl_AbsR'' (qs_schema := ?qs_schema) ?ValidImpl ?r_o ?r_n
+        |- context[CallBagMethod (BagIndexKeys := ?Index') ?ridx ?midx ?r_o ?d] =>
+        let r_o' := fresh "r_o'" in
+        let AbsR_r_o' := fresh "AbsR_r_o'" in
+        let refines_r_o' := fresh "refines_r_o'" in
+        destruct (@refine_BagImplMethods qs_schema Index' _ ValidImpl r_o r_n ridx H midx d) as [r_o' [refines_r_o' AbsR_r_o']];
+          unfold map_IndexedQS_idx in refines_r_o', AbsR_r_o'; simpl in refines_r_o', AbsR_r_o';
+          setoid_rewrite refines_r_o'; simpl in *; simplify with monad laws; simpl
+
+      | H : Build_IndexedQueryStructure_Impl_AbsR'' (qs_schema := ?qs_schema) ?ValidImpl ?r_o ?r_n
+        |- context[Join_Lists (As := ?As) (f := ?f) (a := ?a) ?l ?c ] =>
+        makeEvar (ilist f As -> list (f a))
+                 ltac:(fun c' =>
+                         let refines_c' := fresh in
+                         assert (forall a', refine (c a') (ret (c' a'))) as refines_c';
+                       [intros; try implement_bag_methods
+                       | setoid_rewrite (Join_Lists_Impl l c c' refines_c');
+                         simpl in *; setoid_rewrite (refineEquiv_bind_unit);
+                         implement_bag_methods
+                       ])
+
     end.
+
+
+Ltac FullySharpenQueryStructure qs_schema Index :=
+  let delegateSigs := constr:(Build_IndexedQueryStructure_Impl_Sigs Index) in
+  let delegateSpecs := constr:(Build_IndexedQueryStructure_Impl_Specs Index) in
+  let cRep' := constr:(Build_IndexedQueryStructure_Impl_cRep Index) in
+  let cAbsR' := constr:(@Build_IndexedQueryStructure_Impl_AbsR' qs_schema Index) in
+  match goal with
+      |- Sharpened (@BuildADT ?Rep ?consSigs ?methSigs ?consDefs ?methDefs) =>
+      ilist_of_evar
+        (ilist (fun nadt => ComputationalADT.cADT (namedADTSig nadt)) delegateSigs)
+        (fun DelegateImpl Sig => ComputationalADT.cMethodType (cRep' DelegateImpl) (methDom Sig) (methCod Sig))
+        methSigs
+        ltac:(fun cMeths =>
+                ilist_of_evar
+                  (ilist (fun nadt => ComputationalADT.cADT (namedADTSig nadt)) delegateSigs)
+                  (fun DelegateImpl Sig => ComputationalADT.cConstructorType (cRep' DelegateImpl) (consDom Sig))
+                  consSigs
+                  ltac:(fun cCons =>
+                          eapply
+                            (@Notation_Friendly_SharpenFully
+                               _
+                               consSigs
+                               methSigs
+                               consDefs
+                               methDefs
+                               delegateSigs
+                               cRep'
+                               cCons
+                               cMeths
+                               delegateSpecs
+                               cAbsR')));
+        unfold Dep_Type_BoundedIndex_app_comm_cons
+  end; simpl; intros;
+  [ repeat split; intros; try exact tt; implement_bag_constructors
+  | repeat split; intros; try exact tt; implement_bag_methods ].
